OeufProofIntern QED

src/AllValues.v
@@ -1,81 +1,237 @@
+Require Import List.
+Import ListNotations.
+
+Require SourceValues.
 Require HighestValues.
 Require HigherValue.
 Require HighValues.
 
 Require MatchValues.
 
+Require Import StructTact.StructTactics.
+Require Import StuartTact.
+
 
 Inductive value_level : Set :=
+| VlSource
+        (G : list (SourceValues.type * list SourceValues.type * SourceValues.type))
+        (ty : SourceValues.type)
 | VlHighest
 | VlHigher
+| VlHighFname (* HighValues, using sequential indexes for function names *)
 | VlHigh
 .
 
 
 Definition value_type vl : Type :=
     match vl with
+    | VlSource G ty => SourceValues.value G ty
     | VlHighest => HighestValues.value
     | VlHigher => HigherValue.value
+    | VlHighFname => HighValues.value
     | VlHigh => HighValues.value
     end.
 
+Definition value_match_indexed M vl1 vl2 : value_type vl1 -> value_type vl2 -> Prop :=
+    match vl1, vl2 with
+
+    (* zero steps *)
+    | VlSource G1 ty1, VlSource G2 ty2 =>
+            fun v1 v2 => existT _ G1 (existT _ ty1 v1) = existT _ G2 (existT _ ty2 v2)
+                    :> { G : _ & { ty : _ & SourceValues.value G ty } }
+    | VlHighest, VlHighest => eq
+    | VlHigher, VlHigher => eq
+    | VlHighFname, VlHighFname => eq
+    | VlHigh, VlHigh => eq
+
+    (* one step *)
+    | VlSource G ty, VlHighest => fun v1 v2 => MatchValues.compile_highest v1 = v2
+    | VlHighest, VlHigher => MatchValues.mv_higher
+    | VlHigher, VlHighFname => MatchValues.mv_high
+    | VlHighFname, VlHigh => MatchValues.mv_fmajor M
+
+    (* two steps *)
+    | VlSource G ty, VlHigher => fun v1 v3 => exists v2,
+            MatchValues.compile_highest v1 = v2 /\
+            MatchValues.mv_higher v2 v3
+    | VlHighest, VlHighFname => fun v1 v3 => exists v2,
+            MatchValues.mv_higher v1 v2 /\
+            MatchValues.mv_high v2 v3
+    | VlHigher, VlHigh => fun v1 v3 => exists v2,
+            MatchValues.mv_high v1 v2 /\
+            MatchValues.mv_fmajor M v2 v3
+
+    (* three steps *)
+    | VlSource G ty, VlHighFname => fun v1 v4 => exists v2 v3,
+            MatchValues.compile_highest v1 = v2 /\
+            MatchValues.mv_higher v2 v3 /\
+            MatchValues.mv_high v3 v4
+    | VlHighest, VlHigh => fun v1 v4 => exists v2 v3,
+            MatchValues.mv_higher v1 v2 /\
+            MatchValues.mv_high v2 v3 /\
+            MatchValues.mv_fmajor M v3 v4
+
+    (* four steps *)
+    | VlSource G ty, VlHigh => fun v1 v5 => exists v2 v3 v4,
+            MatchValues.compile_highest v1 = v2 /\
+            MatchValues.mv_higher v2 v3 /\
+            MatchValues.mv_high v3 v4 /\
+            MatchValues.mv_fmajor M v4 v5
+
+    (* anything else *)
+    | _, _ => fun _ _ => False
+    end.
+
+(* Like value_match_indexed, but all cases usind indices are deleted. *)
 Definition value_match vl1 vl2 : value_type vl1 -> value_type vl2 -> Prop :=
     match vl1, vl2 with
 
     (* zero steps *)
+    | VlSource G1 ty1, VlSource G2 ty2 =>
+            fun v1 v2 => existT _ G1 (existT _ ty1 v1) = existT _ G2 (existT _ ty2 v2)
+                    :> { G : _ & { ty : _ & SourceValues.value G ty } }
     | VlHighest, VlHighest => eq
     | VlHigher, VlHigher => eq
+    | VlHighFname, VlHighFname => eq
     | VlHigh, VlHigh => eq
 
     (* one step *)
+    | VlSource G ty, VlHighest => fun v1 v2 => MatchValues.compile_highest v1 = v2
     | VlHighest, VlHigher => MatchValues.mv_higher
-    | VlHigher, VlHigh => MatchValues.mv_high
+    | VlHigher, VlHighFname => MatchValues.mv_high
 
     (* two steps *)
-    | VlHighest, VlHigh => fun v1 v3 => exists v2,
+    | VlSource G ty, VlHigher => fun v1 v3 => exists v2,
+            MatchValues.compile_highest v1 = v2 /\
+            MatchValues.mv_higher v2 v3
+    | VlHighest, VlHighFname => fun v1 v3 => exists v2,
             MatchValues.mv_higher v1 v2 /\
             MatchValues.mv_high v2 v3
 
+    (* three steps *)
+    | VlSource G ty, VlHighFname => fun v1 v4 => exists v2 v3,
+            MatchValues.compile_highest v1 = v2 /\
+            MatchValues.mv_higher v2 v3 /\
+            MatchValues.mv_high v3 v4
+
+    (* four steps *)
+
     (* anything else *)
     | _, _ => fun _ _ => False
+    end.
+
+Definition value_level_le_indexed vl1 vl2 : Prop :=
+    match vl1, vl2 with
+
+    (* zero steps *)
+    | VlSource G1 ty1, VlSource G2 ty2 => G1 = G2 /\ ty1 = ty2
+    | VlHighest, VlHighest => True
+    | VlHigher, VlHigher => True
+    | VlHighFname, VlHighFname => True
+    | VlHigh, VlHigh => True
+
+    (* one step *)
+    | VlSource _ _, VlHighest => True
+    | VlHighest, VlHigher => True
+    | VlHigher, VlHighFname => True
+    | VlHighFname, VlHigh => True
+
+    (* two steps *)
+    | VlSource _ _, VlHigher => True
+    | VlHighest, VlHighFname => True
+    | VlHigher, VlHigh => True
+
+    (* three steps *)
+    | VlSource _ _, VlHighFname => True
+    | VlHighest, VlHigh => True
+
+    (* four steps *)
+    | VlSource _ _, VlHigh => True
+
+    (* anything else *)
+    | _, _ => False
     end.
 
 Definition value_level_le vl1 vl2 : Prop :=
     match vl1, vl2 with
 
     (* zero steps *)
+    | VlSource G1 ty1, VlSource G2 ty2 => G1 = G2 /\ ty1 = ty2
     | VlHighest, VlHighest => True
     | VlHigher, VlHigher => True
+    | VlHighFname, VlHighFname => True
     | VlHigh, VlHigh => True
 
     (* one step *)
+    | VlSource _ _, VlHighest => True
     | VlHighest, VlHigher => True
-    | VlHigher, VlHigh => True
+    | VlHigher, VlHighFname => True
 
     (* two steps *)
-    | VlHighest, VlHigh => True
+    | VlSource _ _, VlHigher => True
+    | VlHighest, VlHighFname => True
+
+    (* three steps *)
+    | VlSource _ _, VlHighFname => True
+
+    (* four steps *)
 
     (* anything else *)
     | _, _ => False
     end.
 
+Lemma value_match_indexed_compose : forall M vl1 vl2 vl3 v1 v2 v3,
+    value_match_indexed M vl1 vl2 v1 v2 ->
+    value_match_indexed M vl2 vl3 v2 v3 ->
+    value_match_indexed M vl1 vl3 v1 v3.
+destruct vl1, vl2, vl3; intros ? ? ? Hm1 Hm2; simpl in *; subst;
+try fix_existT; repeat (break_exists || break_and);
+try solve [eauto | exfalso; eauto | firstorder congruence].
+Qed.
+
+Lemma value_match_indexed_decompose : forall M vl1 vl2 vl3 v1 v3,
+    value_match_indexed M vl1 vl3 v1 v3 ->
+    value_level_le_indexed vl1 vl2 ->
+    value_level_le_indexed vl2 vl3 ->
+    exists v2, value_match_indexed M vl1 vl2 v1 v2 /\ value_match_indexed M vl2 vl3 v2 v3.
+destruct vl1, vl2, vl3; intros ? ? ? Hle1 Hle2;
+try solve [inversion Hle1 | inversion Hle2];
+simpl in *; repeat (break_exists || break_and); subst; eauto 9.
+Qed.
 
 Lemma value_match_compose : forall vl1 vl2 vl3 v1 v2 v3,
     value_match vl1 vl2 v1 v2 ->
     value_match vl2 vl3 v2 v3 ->
     value_match vl1 vl3 v1 v3.
 destruct vl1, vl2, vl3; intros ? ? ? Hm1 Hm2; simpl in *; subst;
-solve [eauto | exfalso; eauto | congruence].
+try fix_existT; repeat (break_exists || break_and);
+try solve [eauto | exfalso; eauto | firstorder congruence].
 Qed.
 
 Lemma value_match_decompose : forall vl1 vl2 vl3 v1 v3,
     value_match vl1 vl3 v1 v3 ->
-    value_level_le vl1 vl2 ->
-    value_level_le vl2 vl3 ->
+    value_level_le_indexed vl1 vl2 ->
+    value_level_le_indexed vl2 vl3 ->
     exists v2, value_match vl1 vl2 v1 v2 /\ value_match vl2 vl3 v2 v3.
-destruct vl1, vl2, vl3; intros ? ? ? Hle1 Hle2;
-try solve [inversion Hle1 | inversion Hle2];
-simpl in *; eauto.
+destruct vl1, vl2, vl3; intros ? ? Hm Hle1 Hle2;
+try solve [inversion Hle1 | inversion Hle2 | inversion Hm];
+simpl in *; repeat (break_exists || break_and); subst; eauto 9.
+Qed.
+
+Lemma value_level_le_indexed_refl : forall vl,
+    value_level_le_indexed vl vl.
+destruct vl; simpl; eauto.
+Qed.
+
+Lemma value_level_le_indexed_trans : forall vl1 vl2 vl3,
+    value_level_le_indexed vl1 vl2 ->
+    value_level_le_indexed vl2 vl3 ->
+    value_level_le_indexed vl1 vl3.
+destruct vl1, vl2; simpl; try solve [intros ? ?; exfalso; eassumption].
+all: destruct vl3; simpl; try solve [intros ? ?; exfalso; eassumption].
+all: intros; eauto.
+
+firstorder congruence.
 Qed.
 
 Lemma value_level_le_refl : forall vl,
@@ -87,6 +243,37 @@ Lemma value_level_le_trans : forall vl1 vl2 vl3,
     value_level_le vl1 vl2 ->
     value_level_le vl2 vl3 ->
     value_level_le vl1 vl3.
-destruct vl1, vl2, vl3; idtac + exfalso; solve [eauto].
+destruct vl1, vl2; simpl; try solve [intros ? ?; exfalso; eassumption].
+all: destruct vl3; simpl; try solve [intros ? ?; exfalso; eassumption].
+all: intros; eauto.
+
+firstorder congruence.
 Qed.
 
+Lemma value_level_le_add_index : forall vl1 vl2,
+    value_level_le vl1 vl2 ->
+    value_level_le_indexed vl1 vl2.
+destruct vl1, vl2; simpl; intro; eauto.
+Qed.
+
+Lemma value_match_remove_index : forall M vl1 vl2 v1 v2,
+    value_level_le vl1 vl2 ->
+    value_match_indexed M vl1 vl2 v1 v2 ->
+    value_match vl1 vl2 v1 v2.
+intros0 Hvm.
+destruct vl1, vl2; simpl in *; eauto.
+Qed.
+
+Lemma value_match_add_index : forall M vl1 vl2 v1 v2,
+    value_match vl1 vl2 v1 v2 ->
+    value_match_indexed M vl1 vl2 v1 v2.
+intros0 Hvm. intros.
+destruct vl1, vl2; simpl in *; eauto; try solve [exfalso; eauto].
+Qed.
+
+Lemma value_match_add_index_iff : forall M vl1 vl2 v1 v2,
+    value_level_le vl1 vl2 ->
+    value_match vl1 vl2 v1 v2 <->
+    value_match_indexed M vl1 vl2 v1 v2.
+intros; split; eauto using value_match_add_index, value_match_remove_index.
+Qed.
