src/MixSemantics.v
@@ -3,8 +3,10 @@ Require Import Relations.
 Require Import Wellfounded.
 
 (* Oeuf *)
-Require Import Semantics.
-Require Import TraceSemantics.
+Require Import FullSemantics.
+Require TraceSemantics.
+Require Semantics.
+Require Import MatchValues AllValues.
 
 (* Compcert *)
 (*Require Import compcert.common.Smallstep.*)
@@ -17,277 +19,216 @@ Require Import StructTact.StructTactics.
 Require Import StructTact.Util.
 
 Require Import EricTact.
+Require Import StuartTact.
+
+Set Implicit Arguments.
 
 
-Definition trace_semantics := TraceSemantics.semantics.
-Definition notrace_semantics := Semantics.semantics.
+Definition forward_simulation L1 L2 M :=
+    FullSemantics.forward_simulation (Semantics.lift L1) L2 M.
 
-Definition trace_fsim_index := fsim_index.
-Definition trace_fsim_order := fsim_order.
 
-Definition trace_forward_simulation := TraceSemantics.forward_simulation.
-Definition notrace_forward_simulation := Semantics.forward_simulation.
+Notation " 'Step1' L " := (Semantics.step L (Semantics.globalenv L)) (at level 1).
+Notation " 'Star1' L " := (Semantics.star (Semantics.step L) (Semantics.globalenv L)) (at level 1).
+Notation " 'Plus1' L " := (Semantics.plus (Semantics.step L) (Semantics.globalenv L)) (at level 1).
 
-(* We need a simulation from notrace to trace *)
-Record mix_forward_simulation (L1 : notrace_semantics) (L2 : trace_semantics) : Type :=
-  Forward_simulation {
-    fsim_index: Type;
-    fsim_order: fsim_index -> fsim_index -> Prop;
-    fsim_order_wf: well_founded fsim_order;
-    fsim_match_states :> fsim_index -> Semantics.state L1 -> state L2 -> Prop;
-    fsim_match_val : Semantics.valtype L1 -> valtype L2 -> Prop;
-    fsim_match_callstate :
+Notation " 'Step2' L " := (TraceSemantics.step L (TraceSemantics.globalenv L)) (at level 1).
+Notation " 'Star2' L " := (TraceSemantics.star (TraceSemantics.step L) (TraceSemantics.globalenv L)) (at level 1).
+Notation " 'Plus2' L " := (TraceSemantics.plus (TraceSemantics.step L) (TraceSemantics.globalenv L)) (at level 1).
+
+
+
+Section FORWARD_SIMU_DIAGRAMS.
+
+Variable L1: Semantics.semantics.
+Variable L2: TraceSemantics.semantics.
+Variable M: id_map.
+
+Let L1' := Semantics.lift L1.
+
+(*Hypothesis public_preserved:
+  forall id, Senv.public_symbol (symbolenv L2) id = Senv.public_symbol (symbolenv L1) id. *)
+
+Variable match_states: state L1' -> state L2 -> Prop.
+Variable match_values: valtype L1' -> valtype L2 -> Prop.
+
+Hypothesis match_callstate :
       forall fv1 av1 fv2 av2 s2,
         is_callstate L2 fv2 av2 s2 ->
-        fsim_match_val fv1 fv2 ->
-        fsim_match_val av1 av2 ->
-        exists s1 i,
-          fsim_match_states i s1 s2 /\
-          Semantics.is_callstate L1 fv1 av1 s1;
-    fsim_match_final_states:
-      forall i s1 s2 v1,
-        fsim_match_states i s1 s2 ->
-        Semantics.final_state L1 s1 v1 ->
-        exists v2,
-          final_state L2 s2 v2 /\ fsim_match_val v1 v2;
-    fsim_simulation:
-      forall s1 s1', Semantics.step L1 (Semantics.globalenv L1) s1 s1' ->
-      forall i s2, fsim_match_states i s1 s2 ->
-      exists i', exists s2',
-         (Plus L2 s2 Events.E0 s2' \/ (Star L2 s2 Events.E0 s2' /\ fsim_order i' i))
-      /\ fsim_match_states i' s1' s2'
-    (* fsim_public_preserved:
-      forall id, Senv.public_symbol (symbolenv L2) id = Senv.public_symbol (Semantics.symbolenv L1) id *)
-    }.
+        match_values fv1 fv2 ->
+        match_values av1 av2 ->
+        exists s1,
+          match_states s1 s2 /\
+          is_callstate L1' fv1 av1 s1.
 
 
-(* Turn a mixed simulation into a sequence of steps *)
-Section SIMULATION_SEQUENCES.
+Hypothesis match_final_states:
+  forall s1 s2 v,
+  match_states s1 s2 ->
+  final_state L1' s1 v ->
+  exists v',
+    final_state L2 s2 v' /\ match_values v v'.
 
-Variable L1: notrace_semantics.
-Variable L2: trace_semantics.
-Variable S: mix_forward_simulation L1 L2.
+Hypothesis fsim_val_level_le :
+    value_level_le_indexed (val_level L1') (val_level L2).
 
-Lemma simulation_star:
-  forall s1 s1',
-    @Semantics.star (Semantics.genvtype L1) (Semantics.state L1) (Semantics.step L1) (Semantics.globalenv L1) s1 s1' ->
-  forall i s2, S i s1 s2 ->
-  exists i', exists s2', Star L2 s2 Events.E0 s2' /\ S i' s1' s2'.
+Hypothesis match_val_canon :
+    forall v1 v2,
+    match_values v1 v2 <->
+    value_match_indexed M (val_level L1') (val_level L2) v1 v2.
+
+
+Ltac assumption_harder := on _, fun H => exact H.
+
+
+Section SIMULATION_STAR_WF.
+
+(** [order] is a well-founded ordering associated with states
+  of the first semantics.  Stuttering steps must correspond
+  to states that decrease w.r.t. [order]. *)
+
+Variable order: state L1' -> state L1' -> Prop.
+Hypothesis order_wf: well_founded order.
+
+Hypothesis simulation:
+  forall s1 s1', Step1 L1 s1 s1' ->
+  forall s2, match_states s1 s2 ->
+  exists s2',
+  (Plus2 L2 s2 E0 s2' \/ (Star2 L2 s2 E0 s2' /\ order s1' s1))
+  /\ match_states s1' s2'.
+
+Lemma forward_simulation_star_wf: forward_simulation L1 L2 M.
 Proof.
-  induction 1; intros.
-  exists i; exists s2; split; auto. apply star_refl.
-  exploit fsim_simulation; eauto. intros [i' [s2' [A B]]].
-  exploit IHstar; eauto. intros [i'' [s2'' [C D]]].
-  exists i''; exists s2''; split; auto. eapply star_trans; eauto.
-  2: instantiate (1 := E0); reflexivity.
-  intuition. apply plus_star; auto.
-Qed.
-
-Lemma fsim_simulation' :
-  forall i (s1 : Semantics.state L1) 
-         (s1' : Semantics.state L1),
-    @Semantics.step L1 (@Semantics.globalenv L1)  s1 s1' ->
-    forall s2,
-      S i s1 s2 ->
-      (exists i' s2', Plus L2 s2 E0 s2' /\ S i' s1' s2') \/
-      (exists i', fsim_order L1 L2 S i' i /\ S i' s1' s2).
-Proof.
-  intros. exploit fsim_simulation; eauto.
-  intros [i' [s2' [A B]]]. intuition.
-  left; exists i'; exists s2'; auto.
-  inv H2.
-  right; exists i'; auto.
-  left; exists i'; exists s2'; split; auto. econstructor; eauto.
-Qed.
-
-
-Lemma simulation_plus:
-  forall s1 s1',
-    @Semantics.plus (Semantics.genvtype L1) (Semantics.state L1) (Semantics.step L1) (Semantics.globalenv L1) s1 s1' ->
-  forall i s2, S i s1 s2 ->
-  (exists i', exists s2', Plus L2 s2 E0 s2' /\ S i' s1' s2')
-  \/ (exists i', clos_trans _ (fsim_order L1 L2 S) i' i /\ S i' s1' s2).
-Proof.
-  induction 1 using Semantics.plus_ind2; intros.
-(* base case *)
-  exploit fsim_simulation'; eauto.
-  intros [A | [i' A]].
-  left; auto. 
-  right; exists i'; intuition.
-(* inductive case *)
-  exploit fsim_simulation'; eauto. intros [[i' [s2' [A B]]] | [i' [A B]]].
-  exploit simulation_star.
-  apply Semantics.plus_star; eauto. eauto.
-  intros [i'' [s2'' [P Q]]].
-  left; exists i''; exists s2''; split; auto. eapply plus_star_trans; eauto.
-  exploit IHplus; eauto.
-  intros [[i'' [s2'' [P Q]]] | [i'' [P Q]]].
-  subst. simpl. left; exists i''; exists s2''; auto.
-  subst. simpl. right; exists i''; intuition.
-  eapply t_trans; eauto. eapply t_step; eauto.
-Qed.
-
-
-
-End SIMULATION_SEQUENCES.
-
-
-
-Section COMPOSE_SIMULATIONS.
-
-Section COMPOSE_NOTRACE_MIX.
-  
-Variable L1: notrace_semantics.
-Variable L2: notrace_semantics.
-Variable L3: trace_semantics.
-Variable S12: notrace_forward_simulation L1 L2.
-Variable S23: mix_forward_simulation L2 L3.
-
-Let ff_index : Type := (fsim_index _ _ S23 * Semantics.fsim_index _ _ S12)%type.
-
-Let ff_order : ff_index -> ff_index -> Prop :=
-  lex_ord (clos_trans _ (fsim_order _ _ S23)) (Semantics.fsim_order _ _ S12).
-
-Let ff_match_states (i: ff_index) (s1: Semantics.state L1) (s3: state L3) : Prop :=
-  exists s2, S12 (snd i) s1 s2 /\ S23 (fst i) s2 s3.
-
-Let ff_match_values (v1 : Semantics.valtype L1) (v3 : valtype L3) : Prop :=
-  exists v2, Semantics.fsim_match_val L1 L2 S12 v1 v2 /\ fsim_match_val L2 L3 S23 v2 v3.
-
-Lemma compose_notrace_mix_forward_simulation: mix_forward_simulation L1 L3.
-Proof.
-  apply Forward_simulation with (fsim_order := ff_order) (fsim_match_states := ff_match_states)
-  (fsim_match_val := ff_match_values).
-(* well founded *)
-  unfold ff_order. apply wf_lex_ord. apply wf_clos_trans. apply fsim_order_wf.
-  apply Semantics.fsim_order_wf.
-(* initial states *)
-  intros. subst ff_match_values. simpl in *. repeat break_exists. repeat break_and.
-  eapply (fsim_match_callstate L2 L3 S23) in H; eauto.
-  repeat break_exists; break_and.
-  eapply (Semantics.fsim_match_callstate L1 L2 S12) in H4; eauto.
-  break_exists; break_and.
-  exists x3. exists (x2,x4). split; eauto.
-  econstructor; eauto.
-(* final states *)
-  intros. destruct H as [s3 [A B]].
-  app (Semantics.fsim_match_final_states L1 L2 S12) Semantics.final_state.
-  app (fsim_match_final_states L2 L3 S23) (Semantics.final_state L2).
-  eexists; split; try econstructor; eauto.
-(* simulation *)
-  intros. destruct H0 as [s3 [A B]]. destruct i as [i2 i1]; simpl in *.
-  exploit (Semantics.fsim_simulation' _ _ S12); eauto. intros [[i1' [s3' [C D]]] | [i1' [C D]]].
-  (* L2 makes one or several steps. *)
-  exploit simulation_plus; eauto. intros [[i2' [s2' [P Q]]] | [i2' [P Q]]].
-  (* L3 makes one or several steps *)
-  exists (i2', i1'); exists s2'; split. auto. exists s3'; auto.
-  (* L3 makes no step *)
-  exists (i2', i1'); exists s2; split.
-  right; split. apply star_refl. red. left. auto.
-  exists s3'; auto.
-  (* L2 makes no step *)
-  exists (i2, i1'); exists s2; split.
-  right; split. apply star_refl. red. right. auto.
-  exists s3; auto.
-(* symbols *)
-(*  intros. transitivity (Senv.public_symbol (Semantics.symbolenv L2) id);
-  try apply fsim_public_preserved; auto;
-  try apply Semantics.fsim_public_preserved; auto. *)
-Defined.
-
-End COMPOSE_NOTRACE_MIX.
-
-Section COMPOSE_MIX_TRACE.
-  
-Variable L1: notrace_semantics.
-Variable L2: trace_semantics.
-Variable L3: trace_semantics.
-Variable S12: mix_forward_simulation L1 L2.
-Variable S23: trace_forward_simulation L2 L3.
-
-Let ff_index : Type := (trace_fsim_index _ _ S23 * fsim_index _ _ S12)%type.
-
-Let ff_order : ff_index -> ff_index -> Prop :=
-  lex_ord (clos_trans _ (trace_fsim_order _ _ S23)) (fsim_order _ _ S12).
-
-Let ff_match_states (i: ff_index) (s1: Semantics.state L1) (s3: state L3) : Prop :=
-  exists s2, S12 (snd i) s1 s2 /\ S23 (fst i) s2 s3.
-
-Let ff_match_values (v1 : Semantics.valtype L1) (v3 : valtype L3) : Prop :=
-  exists v2, fsim_match_val L1 L2 S12 v1 v2 /\ TraceSemantics.fsim_match_val S23 v2 v3.
-
-Lemma compose_mix_trace_forward_simulation: mix_forward_simulation L1 L3.
-Proof.
-  apply Forward_simulation with (fsim_order := ff_order) (fsim_match_states := ff_match_states)
-                                                         (fsim_match_val := ff_match_values).
-(* well founded *)
-  unfold ff_order. apply wf_lex_ord. apply wf_clos_trans.
-  apply TraceSemantics.fsim_order_wf.
-  apply fsim_order_wf.  
-(* initial states *)
-  intros. subst ff_match_values. simpl in *. repeat break_exists. repeat break_and.
-  eapply (TraceSemantics.fsim_match_callstate S23) in H; eauto.
-  repeat break_exists; break_and.
-  eapply (fsim_match_callstate L1 L2 S12) in H4; eauto.
-  break_exists; break_and.
-  exists x3. exists (x2,x4). split; eauto.
-  econstructor; eauto.
-(* final states *)
-  intros. destruct H as [s3 [A B]].
-  app (fsim_match_final_states L1 L2 S12) Semantics.final_state.
-  app (TraceSemantics.fsim_match_final_states S23) (final_state L2).
-  eexists; split; try econstructor; eauto.
-(* simulation *)
-  intros. destruct H0 as [s3 [A B]]. destruct i as [i2 i1]; simpl in *.
-  exploit (fsim_simulation' _ _ S12); eauto. intros [[i1' [s3' [C D]]] | [i1' [C D]]].
-  (* L2 makes one or several steps. *)
-  exploit TraceSemantics.simulation_plus; eauto. intros [[i2' [s2' [P Q]]] | [i2' [P Q]]].
-  (* L3 makes one or several steps *)
-  exists (i2', i1'); exists s2'; split. auto. exists s3'; auto.
-  (* L3 makes no step *)
-  exists (i2', i1'); exists s2; split.
-  right; split. apply star_refl. red. left. auto.
-  exists s3'; auto.
-  simpl. break_and. split; assumption.
-  (* L2 makes no step *)
-  exists (i2, i1'); exists s2; split.
-  right; split. apply star_refl. red. right. auto.
-  exists s3; auto.
-(* symbols *)
-(*  intros.
-  transitivity (Senv.public_symbol (symbolenv L2) id);
-  try apply fsim_public_preserved; auto;
-  try apply TraceSemantics.fsim_public_preserved; auto. *)
-Defined.
-  
-End COMPOSE_MIX_TRACE.
-
-End COMPOSE_SIMULATIONS.
-
-Lemma mix_trace_fsim_match_val_compose :
-  forall sema semb semc fs1 fs2 R1 R2,
-    (forall x y, fsim_match_val sema semb fs1 x y <-> R1 x y) ->
-    (forall x y, TraceSemantics.fsim_match_val fs2 x y <-> R2 x y) ->
-    (forall x y, fsim_match_val sema semc (compose_mix_trace_forward_simulation sema semb semc fs1 fs2) x y <-> (exists z, R1 x z /\ R2 z y)).
-Proof.
-  intros. unfold compose_mix_trace_forward_simulation.
-  simpl. split; intros; repeat (break_exists; break_and);
-           repeat rewrite H in *; repeat rewrite H0 in *.
+  eapply FullSemantics.forward_simulation_star_wf with
+    (order := order)
+    (match_values := match_values)
+    (match_states := match_states);
   eauto.
-  exists x0. split.
-  eapply H; eauto. eapply H0; eauto.
+
+  intros.
+  fwd eapply Semantics.lift_notrace_step; try assumption_harder.
+  subst t.
+  eapply simulation; eauto.
+  unfold L1' in *. simpl in *. break_and. assumption.
 Qed.
 
-Lemma notrace_mix_fsim_match_val_compose :
-  forall sema semb semc fs1 fs2 R1 R2,
-    (forall x y, Semantics.fsim_match_val sema semb fs1 x y <-> R1 x y) ->
-    (forall x y, fsim_match_val semb semc fs2 x y <-> R2 x y) ->
-    (forall x y, fsim_match_val sema semc (compose_notrace_mix_forward_simulation sema semb semc fs1 fs2) x y <-> (exists z, R1 x z /\ R2 z y)).
+End SIMULATION_STAR_WF.
+
+Section SIMULATION_STAR.
+
+(** We now consider the case where we have a nonnegative integer measure
+  associated with states of the first semantics.  It must decrease when we take
+  a stuttering step. *)
+
+Variable measure: state L1' -> nat.
+
+Hypothesis simulation:
+  forall s1 s1', Step1 L1 s1 s1' ->
+  forall s2, match_states s1 s2 ->
+  (exists s2', Plus2 L2 s2 E0 s2' /\ match_states s1' s2')
+  \/ (measure s1' < measure s1 /\ match_states s1' s2)%nat.
+
+Lemma forward_simulation_star: forward_simulation L1 L2 M.
 Proof.
-  intros. unfold compose_notrace_mix_forward_simulation.
-  simpl. split; intros; repeat (break_exists; break_and);
-           repeat rewrite H in *; repeat rewrite H0 in *.
+  eapply FullSemantics.forward_simulation_star with
+    (measure := measure)
+    (match_values := match_values)
+    (match_states := match_states);
   eauto.
-  exists x0. split.
-  eapply H; eauto. eapply H0; eauto.
+
+  intros.
+  fwd eapply Semantics.lift_notrace_step; try assumption_harder.
+  subst t.
+  fwd eapply simulation; eauto.
+    { unfold L1' in *. simpl in *. break_and. eassumption. }
+  tauto.
 Qed.
+
+End SIMULATION_STAR.
+
+(** Simulation when one transition in the first program corresponds
+    to one or several transitions in the second program. *)
+
+Section SIMULATION_PLUS.
+
+Hypothesis simulation:
+  forall s1 s1', Step1 L1 s1 s1' ->
+  forall s2, match_states s1 s2 ->
+  exists s2', Plus2 L2 s2 E0 s2' /\ match_states s1' s2'.
+
+Lemma forward_simulation_plus: forward_simulation L1 L2 M.
+Proof.
+  eapply FullSemantics.forward_simulation_plus with
+    (match_values := match_values)
+    (match_states := match_states);
+  eauto.
+
+  intros.
+  fwd eapply Semantics.lift_notrace_step; try assumption_harder.
+  subst t.
+  eapply simulation; eauto.
+  unfold L1' in *. simpl in *. break_and. assumption.
+Qed.
+
+End SIMULATION_PLUS.
+
+(** Lock-step simulation: each transition in the first semantics
+    corresponds to exactly one transition in the second semantics. *)
+
+Section SIMULATION_STEP.
+
+Hypothesis simulation:
+  forall s1 s1', Step1 L1 s1 s1' ->
+  forall s2, match_states s1 s2 ->
+  exists s2', Step2 L2 s2 E0 s2' /\ match_states s1' s2'.
+
+Lemma forward_simulation_step: forward_simulation L1 L2 M.
+Proof.
+  eapply FullSemantics.forward_simulation_step with
+    (match_values := match_values)
+    (match_states := match_states);
+  eauto.
+
+  intros.
+  fwd eapply Semantics.lift_notrace_step; try assumption_harder.
+  subst t.
+  eapply simulation; eauto.
+  unfold L1' in *. simpl in *. break_and. assumption.
+Qed.
+
+End SIMULATION_STEP.
+
+(** Simulation when one transition in the first program
+    corresponds to zero or one transitions in the second program.
+    However, there is no stuttering: infinitely many transitions
+    in the source program must correspond to infinitely many
+    transitions in the second program. *)
+
+Section SIMULATION_OPT.
+
+Variable measure: state L1' -> nat.
+
+Hypothesis simulation:
+  forall s1 s1', Step1 L1 s1 s1' ->
+  forall s2, match_states s1 s2 ->
+  (exists s2', Step2 L2 s2 E0 s2' /\ match_states s1' s2')
+  \/ (measure s1' < measure s1 /\ match_states s1' s2)%nat.
+
+Lemma forward_simulation_opt: forward_simulation L1 L2 M.
+Proof.
+  eapply FullSemantics.forward_simulation_opt with
+    (match_values := match_values)
+    (match_states := match_states);
+  eauto.
+
+  intros.
+  fwd eapply Semantics.lift_notrace_step; try assumption_harder.
+  subst t.
+  fwd eapply simulation; eauto.
+    { unfold L1' in *. simpl in *. break_and. eassumption. }
+  repeat progress (break_exists || break_and || break_or); eauto.
+Qed.
+
+End SIMULATION_OPT.
+
+End FORWARD_SIMU_DIAGRAMS.
