src/OeufProofIntern.v
@@ -1,24 +1,17 @@
 Require Import OeufIntern.
-Require TopLevel.
 Require Import CompilationUnit.
 Require Import HList.
 Require Import StepLib.
-Require Import MixSemantics.
 Require Import CompilerUtil.
 
 Require Import SourceLifted.
 Require Import HighValues.
+Require Import AllValues.
 
 Require Untyped1.
 Require UntypedComp1.
 Require UntypedCompCombined.
-Require TaggedComp.
-Require TaggedNumberedComp.
-Require ElimFuncComp.
-Require ElimFuncComp2.
-Require ElimFuncComp3.
-Require SwitchedComp.
-Require SelfCloseComp.
+Require ElimFuncCompCombined.
 Require StackCompCombined.
 Require LocalsCompCombined.
 Require FlatCompCombined.
@@ -32,7 +25,8 @@ Require Cmajortominor.
 
 
 Require Import Cmajor. (* Cminor bridge *)
-Require Import TraceSemantics.
+Require FullSemantics.
+Require Semantics.
 
 Require Import compcert.lib.Coqlib.
 Require Import compcert.ia32.Asm.
@@ -49,7 +43,8 @@ Require Import StructTact.Util.
 Require Import EricTact.
 Require Import StuartTact.
 Require Import ListLemmas.
-Require Import Monads.  
+
+Set Default Timeout 15.
 
 
 Lemma transf_oeuf_to_untyped1_genv : forall prog tprog,
@@ -57,7 +52,8 @@ Lemma transf_oeuf_to_untyped1_genv : forall prog tprog,
     UntypedComp1.compile_genv (CompilationUnit.exprs prog) = fst tprog.
 intros. unfold transf_oeuf_to_untyped1 in *.
 break_result_chain.
-simpl in *. subst. simpl in *. break_if; try discriminate. inject_some. simpl.
+simpl in *. break_match; try discriminate. inject_some.
+simpl in *. break_match; try discriminate. inject_some.
 reflexivity.
 Qed.
 
@@ -70,1200 +66,124 @@ unfold Metadata.check_length in *. do 2 (break_match; try discriminate).
 inject_some. auto.
 Qed.
 
+Lemma init_metadata'_public : forall names nfrees,
+    Forall (fun m => Metadata.m_access m = Metadata.Public) (init_metadata' names nfrees).
+induction names; destruct nfrees; simpl in *; try solve [constructor].
+econstructor; eauto.
+Qed.
+
 Lemma transf_oeuf_to_untyped1_meta_public : forall prog tprog,
     transf_oeuf_to_untyped1 prog = OK tprog ->
     Forall (fun m => Metadata.m_access m = Metadata.Public) (snd tprog).
 intros. unfold transf_oeuf_to_untyped1 in *.
 break_result_chain.
 simpl in *; eauto.
-unfold Metadata.check_length in *. do 2 (break_match; try discriminate).
-inject_some. inject_pair. simpl.
-eapply Forall_map. rewrite Forall_forall.
-intros. simpl. reflexivity.
+unfold Metadata.check_length in *. do 3 (break_match; try discriminate).
+inject_some. simpl.
+eapply init_metadata'_public.
 Qed.
 
+Lemma transf_oeuf_to_untyped1_nfree : forall prog tprog,
+    transf_oeuf_to_untyped1 prog = OK tprog ->
+    Forall2 (fun g m => Metadata.m_nfree m = g_nfree g) (types prog) (snd tprog).
+intros. unfold transf_oeuf_to_untyped1 in *.
+break_result_chain.
+simpl in *. break_match; try discriminate. inject_some.
+simpl in *. break_match; try discriminate. inject_some.
+eauto.
+Qed.
 
-Section ComposeSourceLifted.
-
-    Variable P1 : CompilationUnit.compilation_unit.
-    Let G := CompilationUnit.types P1.
-    Let g := CompilationUnit.exprs P1.
-
-    Variable P2 : Untyped1.prog_type.
-    Let L2 : Semantics.semantics := Untyped1.semantics P2.
-
-    Variable L3 : TraceSemantics.semantics.
-
-    Hypothesis TRANSF12 : transf_oeuf_to_untyped1 P1 = OK P2.
-    Variable S23 : mix_forward_simulation L2 L3.
-
-
-    Let ff_index : Type := MixSemantics.fsim_index _ _ S23.
-    Let ff_order : ff_index -> ff_index -> Prop := MixSemantics.fsim_order _ _ S23.
-
-    Let ff_match_states {rty}
-            (i : ff_index)
-            (s1 : SourceLifted.state G rty)
-            (s3 : TraceSemantics.state L3) :=
-        exists s2,
-            UntypedComp1.compile_state s1 = s2 /\
-            S23 i s2 s3.
-
-    Let ff_match_values {ty}
-            (v1 : SourceLifted.value G ty)
-            (v3 : TraceSemantics.valtype L3) :=
-        exists v2,
-            UntypedComp1.compile_value v1 = v2 /\
-            MixSemantics.fsim_match_val _ _ S23 v2 v3.
-
-    Definition sl_index := ff_index.
-    Definition sl_order := ff_order.
-    Definition sl_match_states {rty} := @ff_match_states rty.
-    Definition sl_match_values {ty} := @ff_match_values ty.
-
-    Lemma sl_match_callstate :
-        forall tyA tyR
-            (fv1 : SourceLifted.value G (SourceLifted.Arrow tyA tyR))
-            (av1 : SourceLifted.value G tyA)
-            (fv3 av3 : TraceSemantics.valtype L3)
-            (s3 : TraceSemantics.state L3),
-        TraceSemantics.is_callstate L3 fv3 av3 s3 ->
-        ff_match_values fv1 fv3 ->
-        ff_match_values av1 av3 ->
-        exists s1 i,
-            ff_match_states i s1 s3 /\
-            SourceLifted.is_callstate g fv1 av1 s1.
-    intros0 Hcs Hmv_f Hmv_a.
-    destruct Hmv_f as (fv2 & ? & ?).
-    destruct Hmv_a as (av2 & ? & ?).
-
-    fwd eapply (MixSemantics.fsim_match_callstate _ _ S23) as HH; eauto.
-      destruct HH as (s2 & i & ? & ?).
-
-    destruct P2 as [P2env P2meta].
-    fwd eapply transf_oeuf_to_untyped1_genv; eauto. simpl in *.
-    fwd eapply UntypedComp1.match_callstate as HH; eauto.
-      destruct HH as (s1 & ? & ?).
-
-    unfold ff_match_states. eauto 7.
-    Qed.
-
-    Lemma sl_match_final_states :
-        forall ty i
-            (s1 : SourceLifted.state G ty)
-            (s3 : TraceSemantics.state L3)
-            (v1 : SourceLifted.value G ty),
-        ff_match_states i s1 s3 ->
-        SourceLifted.final_state s1 v1 ->
-        exists v3,
-            TraceSemantics.final_state L3 s3 v3 /\
-            ff_match_values v1 v3.
-    intros0 Hms Hfin.
-    destruct Hms as (s2 & ? & ?).
-
-    destruct P2 as [P2env P2meta].
-    fwd eapply transf_oeuf_to_untyped1_genv; eauto. simpl in *.
-    fwd eapply transf_oeuf_to_untyped1_meta_len; eauto.
-    fwd eapply transf_oeuf_to_untyped1_meta_public; eauto.
-    simpl in *.
-
-    fwd eapply UntypedComp1.match_final_state with (Bmeta := P2meta) as HH; eauto.
-      destruct HH as (v2 & ? & ?).
-
-    fwd eapply (MixSemantics.fsim_match_final_states _ _ S23) as HH; eauto.
-      destruct HH as (v3 & ? & ?).
-
-    unfold ff_match_values. eauto.
-    Qed.
-
-
-    Lemma sl_simulation :
-        forall rty (s1 s1' : SourceLifted.state G rty),
-        SourceLifted.sstep g s1 s1' ->
-        forall i s3,
-        ff_match_states i s1 s3 ->
-        exists i', exists s3',
-            ((TraceSemantics.plus
-                    (TraceSemantics.step L3)
-                    (TraceSemantics.globalenv L3)
-                    s3 Events.E0 s3') \/
-                (TraceSemantics.star
-                        (TraceSemantics.step L3)
-                        (TraceSemantics.globalenv L3)
-                        s3 Events.E0 s3' /\
-                    ff_order i' i)) /\
-            ff_match_states i' s1' s3'.
-    intros0 Hstep. intros0 Hmatch.
-    destruct Hmatch as (s2 & ? & ?).
-
-    destruct P2 as [P2env P2meta].
-    fwd eapply transf_oeuf_to_untyped1_genv; eauto. simpl in *.
-    fwd eapply transf_oeuf_to_untyped1_meta_len; eauto.
-    fwd eapply transf_oeuf_to_untyped1_meta_public; eauto.
-    simpl in *.
-
-    fwd eapply UntypedComp1.I_sim as HH; eauto.
-      destruct HH as (s2' & ? & ?).
-
-    fwd eapply (MixSemantics.fsim_simulation _ _ S23) as HH; eauto.
-      destruct HH as (i' & s3' & ? & ?).
-
-    unfold ff_match_states. eauto 7.
-    Qed.
-
-    (* TODO: backward sim? *)
-
-End ComposeSourceLifted.
-
-Section FSIMtagged.
-
-  Variable a : Untyped1.prog_type.
-  Variable b : Tagged.prog_type.
-  Hypothesis TRANSF : transf_untyped_to_tagged a = OK b.
-
-  Lemma compile_tagged_succ :
-    { c | UntypedCompCombined.compile_cu a = Some c }.
-  Proof.
-    unfold transf_untyped_to_tagged in TRANSF. break_result_chain. eauto.
-  Qed.
-  
-  Definition fsim_tagged : Semantics.forward_simulation (Untyped1.semantics a) (Tagged.semantics b).
-    destruct compile_tagged_succ.
-    eapply Semantics.compose_forward_simulation;
-      try eapply UntypedCompCombined.fsim; eauto;
-      try eapply TaggedComp.fsim; eauto.
-    unfold transf_untyped_to_tagged in *; break_result_chain.
-    try unfold option_to_res in *.
-    congruence.
-  Defined.
-
-  Lemma fsim_tagged_match_val :
-    forall x y,
-      Semantics.fsim_match_val _ _ fsim_tagged x y <-> TaggedComp.I_value x y.
-  Proof.
-    intros. unfold fsim_tagged.
-    destruct compile_tagged_succ.
-    erewrite Semantics.fsim_match_val_compose.
-    Focus 2. intros. erewrite UntypedCompCombined.fsim_match_val.
-    split; intros; congruence.
-    instantiate (1 := MatchValues.mv_higher).
-    split; intros; repeat break_exists; repeat break_and;
-      try erewrite UntypedCompCombined.fsim_match_val in *.
-    congruence. eexists; split. 
-    eapply UntypedCompCombined.fsim_match_val. reflexivity. assumption.
-    simpl.
-    intros.
-    erewrite TaggedComp.match_val_I. reflexivity.
-  Qed.
-
-End FSIMtagged.
-
-Section FSIMtaggednumbered.
-
-  Variable a : Untyped1.prog_type.
-  Variable b : TaggedNumbered.prog_type.
-  Hypothesis TRANSF : transf_untyped_to_tagged_numbered a = OK b.
-
-  Lemma compile_taggednumbered_succ :
-    { c | transf_untyped_to_tagged a = Some c }.
-  Proof.
-    unfold transf_untyped_to_tagged_numbered in TRANSF. break_result_chain. eauto.
-  Qed.
-  
-  Definition fsim_taggednumbered : Semantics.forward_simulation (Untyped1.semantics a) (TaggedNumbered.semantics b).
-    destruct compile_taggednumbered_succ.
-    eapply Semantics.compose_forward_simulation;
-    try eapply fsim_tagged; eauto;
-    try eapply TaggedNumberedComp.fsim; eauto.
-    unfold transf_untyped_to_tagged_numbered in *; break_result_chain.
-    try unfold option_to_res in *.
-    congruence.
-  Defined.
-
-  Lemma fsim_taggednumbered_match_val :
-    forall x y,
-      Semantics.fsim_match_val _ _ fsim_taggednumbered x y <-> TaggedComp.I_value x y.
-  Proof.
-    intros. unfold fsim_taggednumbered.
-    destruct compile_taggednumbered_succ.
-    erewrite Semantics.fsim_match_val_compose.
-    Focus 2. eapply fsim_tagged_match_val; eauto.
-    instantiate (1 := eq).
-    split; intros; repeat break_exists; repeat break_and; try eexists; try split; try eassumption; try congruence.
-    erewrite TaggedNumberedComp.match_val_eq.
-    split; intros; congruence.
-  Qed.
-
-End FSIMtaggednumbered.
-
-
-Section FSIMelimfunc.
-
-  Variable a : Untyped1.prog_type.
-  Variable b : ElimFunc.prog_type.
-  Hypothesis TRANSF : transf_untyped_to_elim_func a = OK b.
-
-  Lemma compile_elimfunc_succ :
-    { c | transf_untyped_to_tagged_numbered a = Some c }.
-  Proof.
-    unfold transf_untyped_to_elim_func in TRANSF. break_result_chain. eauto.
-  Qed.
-  
-  Definition fsim_elimfunc : Semantics.forward_simulation (Untyped1.semantics a) (ElimFunc.semantics b).
-    destruct compile_elimfunc_succ.
-    eapply Semantics.compose_forward_simulation;
-    try eapply fsim_taggednumbered; eauto;
-    try eapply ElimFuncComp.fsim; eauto.
-    unfold transf_untyped_to_elim_func in *; break_result_chain.
-    try unfold option_to_res in *.
-    congruence.
-    unfold transf_untyped_to_tagged_numbered in *.
-    break_result_chain. inv e.
-    eapply TaggedNumberedComp.compile_cu_elims_match'. 
-    reflexivity.
-  Defined.
-
-  Lemma fsim_elimfunc_match_val :
-    forall x y,
-      Semantics.fsim_match_val _ _ fsim_elimfunc x y <-> TaggedComp.I_value x y.
-  Proof.
-    intros. unfold fsim_elimfunc.
-    destruct compile_elimfunc_succ.
-    erewrite Semantics.fsim_match_val_compose.
-    Focus 2. eapply fsim_taggednumbered_match_val; eauto.
-    instantiate (1 := eq).
-    split; intros; repeat break_exists; repeat break_and; try eexists; try split; try eassumption; try congruence.
-    erewrite ElimFuncComp.match_val_eq.
-    split; intros; congruence.
-  Qed.
-
-End FSIMelimfunc.
-
-Definition match_val_highest_higher {A B l} (hstv : HighestValues.value) (hv : HigherValue.value) : Prop :=
-  exists hv',
-    TaggedComp.I_value hstv hv' /\
-    ElimFuncComp2.match_values A B l hv' hv.
-
-Section MATCH_VAL_INDICES.
-
-  Variable u1p : Untyped1.prog_type.
-  Variable efp : ElimFunc.prog_type.
-  Hypothesis EFTRANSF : transf_untyped_to_elim_func u1p = OK efp.
-  Variable ef2p : ElimFunc2.prog_type.
-  Hypothesis EF2TRANSF : ElimFuncComp2.compile_cu efp = Some ef2p.
-
-  Definition match_vals := @match_val_highest_higher (fst efp) (fst ef2p) (snd efp).
-  
-Section FSIMelimfunc2.
-
-  Definition fsim_elimfunc2 : Semantics.forward_simulation (Untyped1.semantics u1p) (ElimFunc2.semantics ef2p).
-    eapply Semantics.compose_forward_simulation;
-    try eapply fsim_elimfunc; eauto;
-      try eapply ElimFuncComp2.fsim; eauto.
-  Defined.
-
-  Lemma fsim_elimfunc2_match_val :
-    forall x y,
-      Semantics.fsim_match_val _ _ fsim_elimfunc2 x y <-> match_vals x y.
-  Proof.
-    intros. unfold fsim_elimfunc2.
-    erewrite Semantics.fsim_match_val_compose.
-    Focus 2. eapply fsim_elimfunc_match_val; eauto.
-    unfold match_vals.
-    unfold match_val_highest_higher.
-    split; intros; repeat break_exists; repeat break_and; try eexists; try split; try eassumption; try congruence.
-    erewrite ElimFuncComp2.match_val_eq.
-    reflexivity.
-  Qed.
-
-End FSIMelimfunc2.
-
-Section FSIMelimfunc3.
-
-  Variable b : ElimFunc3.prog_type.
-  Hypothesis TRANSF : transf_untyped_to_elim_func3 u1p = OK b.
-  
-  Lemma compile_elimfunc3_succ :
-    { c | transf_untyped_to_elim_func2 u1p = Some c }.
-  Proof.
-    unfold transf_untyped_to_elim_func3 in TRANSF. break_result_chain. eauto.
-  Qed.
-  
-  Definition fsim_elimfunc3 : Semantics.forward_simulation (Untyped1.semantics u1p) (ElimFunc3.semantics b).
-    destruct compile_elimfunc3_succ.
-    eapply Semantics.compose_forward_simulation;
-    try eapply fsim_elimfunc2; eauto;
-    try eapply ElimFuncComp3.fsim; eauto.
-    unfold transf_untyped_to_elim_func3 in *; break_result_chain.
-    try unfold option_to_res in *.
-    unfold transf_untyped_to_elim_func2 in e.
-    break_result_chain. 
-    rewrite EFTRANSF in Heqr0. invc Heqr0.
-    rewrite H0 in EF2TRANSF. invc EF2TRANSF.
-    unfold transf_untyped_to_elim_func2 in Heqr.
-    break_result_chain. congruence.
-  Defined.
-
-  Lemma fsim_elimfunc3_match_val :
-    forall x y,
-      Semantics.fsim_match_val _ _ fsim_elimfunc3 x y <-> match_vals x y.
-  Proof.
-    intros. unfold fsim_elimfunc3.
-    destruct compile_elimfunc3_succ.
-    erewrite Semantics.fsim_match_val_compose.
-    Focus 2. eapply fsim_elimfunc2_match_val; eauto.
-    instantiate (1 := eq).
-
-    split; intros; repeat break_exists; repeat break_and; try subst. assumption.
-    eexists; split. eassumption. reflexivity.
-    
-
-    erewrite ElimFuncComp3.match_val_eq.
-    split; intros; try congruence.
-  Qed.
-
-End FSIMelimfunc3.
-
-Section FSIMswitched.
-
-  Variable b : Switched.prog_type.
-  Hypothesis TRANSF : transf_untyped_to_switched u1p = OK b.
-  
-  Lemma compile_switched_succ :
-    { c | transf_untyped_to_elim_func3 u1p = Some c }.
-  Proof.
-    unfold transf_untyped_to_switched in TRANSF. break_result_chain. eauto.
-  Qed.
-  
-  Definition fsim_switched : Semantics.forward_simulation (Untyped1.semantics u1p) (Switched.semantics b).
-    destruct compile_switched_succ.
-    eapply Semantics.compose_forward_simulation;
-    try eapply fsim_elimfunc3; eauto;
-      try eapply SwitchedComp.fsim; eauto.
-    unfold transf_untyped_to_switched in TRANSF.
-    break_result_chain. rewrite e in Heqr. inv Heqr.
-    congruence.
-  Defined.
-
-  Lemma fsim_switched_match_val :
-    forall x y,
-      Semantics.fsim_match_val _ _ fsim_switched x y <-> match_vals x y.
-  Proof.
-    intros. unfold fsim_switched.
-    destruct compile_switched_succ.
-    erewrite Semantics.fsim_match_val_compose.
-    Focus 2. eapply fsim_elimfunc3_match_val; eauto.
-    instantiate (1 := eq).
-
-    split; intros; repeat break_exists; repeat break_and; try subst. assumption.
-    eexists; split. eassumption. reflexivity.
-    
-
-    erewrite SwitchedComp.match_val_eq.
-    split; intros; try congruence.
-  Qed.
-
-End FSIMswitched.
-
-Section FSIMself_close.
-
-  Variable b : SelfClose.prog_type.
-  Hypothesis TRANSF : transf_untyped_to_self_close u1p = OK b.
-  
-  Lemma compile_self_close_succ :
-    { c | transf_untyped_to_switched u1p = Some c }.
-  Proof.
-    unfold transf_untyped_to_self_close in TRANSF. break_result_chain. eauto.
-  Qed.
-  
-  Definition fsim_self_close : Semantics.forward_simulation (Untyped1.semantics u1p) (SelfClose.semantics b).
-    destruct compile_self_close_succ.
-    eapply Semantics.compose_forward_simulation;
-    try eapply fsim_switched; eauto;
-      try eapply SelfCloseComp.fsim; eauto.
-    unfold transf_untyped_to_self_close in TRANSF.
-    break_result_chain. rewrite e in Heqr. inv Heqr.
-    congruence.
-  Defined.
-
-  Lemma fsim_self_close_match_val :
-    forall x y,
-      Semantics.fsim_match_val _ _ fsim_self_close x y <-> match_vals x y.
-  Proof.
-    intros. unfold fsim_self_close.
-    destruct compile_self_close_succ.
-    erewrite Semantics.fsim_match_val_compose.
-    Focus 2. eapply fsim_switched_match_val; eauto.
-    instantiate (1 := eq).
-
-    split; intros; repeat break_exists; repeat break_and; try subst. assumption.
-    eexists; split. eassumption. reflexivity.
-    
-
-    erewrite SelfCloseComp.match_val_eq.
-    split; intros; try congruence.
-  Qed.
-
-End FSIMself_close.
-
-Section FSIMvalue_flag.
-
-  Variable b : ValueFlag.prog_type.
-  Hypothesis TRANSF : transf_untyped_to_value_flag u1p = OK b.
-  
-  Lemma compile_value_flag_succ :
-    { c | transf_untyped_to_self_close u1p = Some c }.
-  Proof.
-    unfold transf_untyped_to_value_flag in TRANSF. break_result_chain. eauto.
-  Qed.
-  
-  Definition fsim_value_flag : Semantics.forward_simulation (Untyped1.semantics u1p) (ValueFlag.semantics b).
-    destruct compile_value_flag_succ.
-    eapply Semantics.compose_forward_simulation;
-    try eapply fsim_self_close; eauto;
-      try eapply ValueFlagComp.fsim; eauto.
-    unfold transf_untyped_to_value_flag in TRANSF.
-    break_result_chain. rewrite e in Heqr. inv Heqr.
-    congruence.
-  Defined.
-
-  Lemma fsim_value_flag_match_val :
-    forall x y,
-      Semantics.fsim_match_val _ _ fsim_value_flag x y <-> match_vals x y.
-  Proof.
-    intros. unfold fsim_value_flag.
-    destruct compile_value_flag_succ.
-    erewrite Semantics.fsim_match_val_compose.
-    Focus 2. eapply fsim_self_close_match_val; eauto.
-    instantiate (1 := eq).
-
-    split; intros; repeat break_exists; repeat break_and; try subst. assumption.
-    eexists; split. eassumption. reflexivity.
-    
-
-    erewrite ValueFlagComp.match_val_eq.
-    split; intros; try congruence.
-  Qed.
-
-End FSIMvalue_flag.
-
-Section FSIMstack.
-
-  Variable b : StackFlatter2.prog_type.
-  Hypothesis TRANSF : transf_untyped_to_stack u1p = OK b.
-  
-  Lemma compile_stack_succ :
-    { c | transf_untyped_to_value_flag u1p = Some c }.
-  Proof.
-    unfold transf_untyped_to_stack in TRANSF. break_result_chain. eauto.
-  Qed.
-  
-  Definition fsim_stack : Semantics.forward_simulation (Untyped1.semantics u1p) (StackFlatter2.semantics b).
-    destruct compile_stack_succ.
-    eapply Semantics.compose_forward_simulation;
-    try eapply fsim_value_flag; eauto;
-      try eapply StackCompCombined.fsim; eauto.
-    unfold transf_untyped_to_stack in TRANSF.
-    break_result_chain. rewrite e in Heqr. inv Heqr.
-    congruence.
-  Defined.
-
-  Lemma fsim_stack_match_val :
-    forall x y,
-      Semantics.fsim_match_val _ _ fsim_stack x y <-> match_vals x y.
-  Proof.
-    intros. unfold fsim_stack.
-    destruct compile_stack_succ.
-    erewrite Semantics.fsim_match_val_compose.
-    Focus 2. eapply fsim_value_flag_match_val; eauto.
-    instantiate (1 := eq).
-
-    split; intros; repeat break_exists; repeat break_and; try subst. assumption.
-    eexists; split. eassumption. reflexivity.
-    
-    intros.
-    erewrite StackCompCombined.match_val_eq.
-    split; intros; try congruence.
-  Qed.
-
-End FSIMstack.
-
-Section FSIMlocals.
-
-  Variable b : LocalsOnly.prog_type.
-  Hypothesis TRANSF : transf_untyped_to_locals u1p = OK b.
-  
-  Lemma compile_locals_succ :
-    { c | transf_untyped_to_stack u1p = Some c }.
-  Proof.
-    unfold transf_untyped_to_locals in TRANSF. break_result_chain. eauto.
-  Qed.
-  
-  Definition fsim_locals : Semantics.forward_simulation (Untyped1.semantics u1p) (LocalsOnly.semantics b).
-    destruct compile_locals_succ.
-    eapply Semantics.compose_forward_simulation;
-    try eapply fsim_stack; eauto;
-      try eapply LocalsCompCombined.fsim; eauto.
-    unfold transf_untyped_to_locals in TRANSF.
-    break_result_chain. rewrite e in Heqr. inv Heqr.
-    congruence.
-  Defined.
-
-  Lemma fsim_locals_match_val :
-    forall x y,
-      Semantics.fsim_match_val _ _ fsim_locals x y <-> match_vals x y.
-  Proof.
-    intros. unfold fsim_locals.
-    destruct compile_locals_succ.
-    erewrite Semantics.fsim_match_val_compose.
-    Focus 2. eapply fsim_stack_match_val; eauto.
-    instantiate (1 := eq).
-
-    split; intros; repeat break_exists; repeat break_and; try subst. assumption.
-    eexists; split. eassumption. reflexivity.
-    
-    intros.
-    erewrite LocalsCompCombined.match_val.
-    split; intros; try congruence.
-  Qed.
-
-End FSIMlocals.
-
-Definition match_val_highest_high {A B l} (hstv : HighestValues.value) (hv : value) : Prop :=
-  exists hv' hv'',
-    TaggedComp.I_value hstv hv' /\
-    ElimFuncComp2.match_values A B l hv' hv'' /\
-    FlatIntTagComp.I_value hv'' hv.
-
-Definition match_vals2 := @match_val_highest_high (fst efp) (fst ef2p) (snd efp).
-  
-Section FSIMflat.
-
-  Variable b : FlatIntTag.prog_type.
-  Hypothesis TRANSF : transf_untyped_to_flat u1p = OK b.
-  
-  Lemma compile_flat_succ :
-    { c | transf_untyped_to_locals u1p = Some c }.
-  Proof.
-    unfold transf_untyped_to_flat in TRANSF. break_result_chain. eauto.
-  Qed.
-
-  Definition fsim_flat : Semantics.forward_simulation (Untyped1.semantics u1p) (FlatIntTag.semantics b).
-    destruct compile_flat_succ.
-    eapply Semantics.compose_forward_simulation;
-    try eapply fsim_locals; eauto;
-      try eapply FlatCompCombined.fsim; eauto.
-    unfold transf_untyped_to_flat in TRANSF.
-    break_result_chain. rewrite e in Heqr. inv Heqr.
-    congruence.
-  Defined.
-
-  Lemma fsim_flat_match_val :
-    forall x y,
-      Semantics.fsim_match_val _ _ fsim_flat x y <-> match_vals2 x y.
-  Proof.
-    intros. unfold fsim_flat.
-    destruct compile_flat_succ.
-    erewrite Semantics.fsim_match_val_compose.
-    Focus 2. eapply fsim_locals_match_val; eauto.
-    unfold match_vals2. unfold match_val_highest_high. unfold match_vals.
-    unfold match_val_highest_higher.
-    
-    split; intros; repeat progress (try break_exists; try break_and).
-    Focus 2.
-    eexists. split. eexists. split. eassumption.
-    eassumption. eassumption.
-    eexists; eexists; repeat split; eauto.
-
-    intros.
-    erewrite FlatCompCombined.match_val_I_value.
-    split; intros; try congruence.
-  Qed.
-
-End FSIMflat.
-
-Definition match_val_highest_high' {A B l M} (hstv : HighestValues.value) (hv : value) : Prop :=
-  exists hv' hv'' hv0,
-    TaggedComp.I_value hstv hv' /\
-    ElimFuncComp2.match_values A B l hv' hv'' /\
-    FlatIntTagComp.I_value hv'' hv0 /\
-    FmajorComp.I_value M hv0 hv.
-
-Section IDMap.
-
-  Variable M : MatchValues.id_map.
-  
-  Definition match_vals3 := @match_val_highest_high' (fst efp) (fst ef2p) (snd efp) M.
-  
-Section FSIMfmajor.
-
-  Variable fm : Fmajor.program.
-  Hypothesis FMTRANSF : transf_untyped_to_fmajor M u1p = OK fm.
-  
-  Lemma compile_fmajor_succ :
-    { c | transf_untyped_to_flat u1p = Some c }.
-  Proof.
-    unfold transf_untyped_to_fmajor in FMTRANSF. break_result_chain. eauto.
-  Qed.
-  
-  Definition fsim_fmajor : MixSemantics.mix_forward_simulation (Untyped1.semantics u1p) (Fmajor.semantics fm).
-    destruct compile_fmajor_succ.
-    eapply MixSemantics.compose_notrace_mix_forward_simulation;
-    try eapply fsim_flat; eauto;
-      try eapply FmajorComp.fsim; eauto.
-    unfold transf_untyped_to_fmajor in FMTRANSF.
-    unfold transf_untyped_to_flat in *.
-    break_result_chain.
-    rewrite Heqr in Heqr1. inversion Heqr1.
-    subst p.
-    rewrite e in Heqr0. inversion Heqr0.
-    subst x. eassumption.
-  Defined.
-
-  Lemma fsim_fmajor_match_val :
-    forall x y,
-      MixSemantics.fsim_match_val _ _ fsim_fmajor x y <-> match_vals3 x y.
-  Proof.
-    intros. unfold fsim_fmajor.
-    destruct compile_fmajor_succ.
-    erewrite MixSemantics.notrace_mix_fsim_match_val_compose.
-    Focus 2. eapply fsim_flat_match_val; eauto.
-
-    instantiate (1 := FmajorComp.I_value M).
-    unfold match_vals2; unfold match_vals3;
-    unfold match_val_highest_high;
-      unfold match_val_highest_high'.
-    split; intros; repeat progress (try break_exists; try break_and);
-      repeat progress (try eexists; try split);
-      try eassumption; try congruence.
-
-    erewrite FmajorComp.match_val_eq.
-    reflexivity.
-  Qed.
-    
-End FSIMfmajor.
-
-Section FSIMfflatmajor.
-
-  Variable ff : Fflatmajor.program.
-  Hypothesis TRANSF : transf_untyped_to_fflatmajor M u1p = OK ff.
-  
-  Lemma compile_fflatmajor_succ :
-    { c | transf_untyped_to_fmajor M u1p = Some c }.
-  Proof.
-    unfold transf_untyped_to_fflatmajor in TRANSF. break_result_chain. eauto.
-  Qed.
-  
-  Definition fsim_fflatmajor : MixSemantics.mix_forward_simulation (Untyped1.semantics u1p) (Fflatmajor.semantics ff).
-    destruct compile_fflatmajor_succ.
-    eapply MixSemantics.compose_mix_trace_forward_simulation;
-    try eapply fsim_fmajor; eauto;
-      try eapply Fmajortofflatmajor.fsim; eauto.
-    unfold transf_untyped_to_fflatmajor in TRANSF.
-    unfold transf_untyped_to_fmajor in *.
-    break_result_chain. unfold labeled in e.
-    break_match_hyp; try congruence.
-    inv H0. inv e.
-    reflexivity.
-  Defined.
-
-  Lemma fsim_fflatmajor_match_val :
-    forall x y,
-      MixSemantics.fsim_match_val _ _ fsim_fflatmajor x y <-> match_vals3 x y.
-  Proof.
-    intros. unfold fsim_fflatmajor.
-    destruct compile_fflatmajor_succ.
-    erewrite MixSemantics.mix_trace_fsim_match_val_compose.
-    Focus 2. eapply fsim_fmajor_match_val; eauto.
-
-    instantiate (1 := eq).
-    split; intros; try break_exists; try break_and.
-    congruence. eauto.
-
-    erewrite Fmajortofflatmajor.match_val_eq.
-    reflexivity.
-  Qed.
-    
-End FSIMfflatmajor.
-
-Section FSIMemajor.
-
-  Variable em : Emajor.program.
-  Hypothesis TRANSF : transf_untyped_to_emajor M u1p = OK em.
-  
-  Lemma compile_emajor_succ :
-    { c | transf_untyped_to_fflatmajor M u1p = Some c }.
-  Proof.
-    unfold transf_untyped_to_emajor in TRANSF. break_result_chain. eauto.
-  Qed.
-  
-  Definition fsim_emajor : MixSemantics.mix_forward_simulation (Untyped1.semantics u1p) (Emajor.semantics em).
-    destruct compile_emajor_succ.
-    eapply MixSemantics.compose_mix_trace_forward_simulation;
-    try eapply fsim_fflatmajor; eauto;
-      try eapply Fflatmajortoemajor.fsim; eauto.
-    unfold transf_untyped_to_emajor in *.
-    unfold transf_untyped_to_fflatmajor in *.
-    break_result_chain.
-    inv e. congruence.
-  Defined.
-
-  Lemma fsim_emajor_match_val :
-    forall x y,
-      MixSemantics.fsim_match_val _ _ fsim_emajor x y <-> match_vals3 x y.
-  Proof.
-    intros. unfold fsim_emajor.
-    destruct compile_emajor_succ.
-    erewrite MixSemantics.mix_trace_fsim_match_val_compose.
-    Focus 2. eapply fsim_fflatmajor_match_val; eauto.
-
-    instantiate (1 := eq).
-    split; intros; try break_exists; try break_and.
-    congruence. eauto.
-
-    erewrite Fflatmajortoemajor.match_val_eq.
-    reflexivity.
-  Qed.
-    
-End FSIMemajor.
-
-Section FSIMdmajor.
-
-  Variable dm : Dmajor.program.
-  Hypothesis TRANSF : transf_untyped_to_dmajor M u1p = OK dm.
-  
-  Lemma compile_dmajor_succ :
-    { c | transf_untyped_to_emajor M u1p = Some c }.
-  Proof.
-    unfold transf_untyped_to_dmajor in TRANSF. break_result_chain. eauto.
-  Qed.
-  
-  Definition fsim_dmajor : MixSemantics.mix_forward_simulation (Untyped1.semantics u1p) (Dmajor.semantics dm).
-    destruct compile_dmajor_succ.
-    eapply MixSemantics.compose_mix_trace_forward_simulation;
-    try eapply fsim_emajor; eauto;
-      try eapply Emajortodmajor.fsim; eauto.
-    unfold transf_untyped_to_dmajor in *.
-    unfold transf_untyped_to_emajor in *.
-    break_result_chain.
-    inv e. congruence.
-  Defined.
-
-  Lemma fsim_dmajor_match_val :
-    forall x y,
-      MixSemantics.fsim_match_val _ _ fsim_dmajor x y <-> match_vals3 x y.
-  Proof.
-    intros. unfold fsim_dmajor.
-    destruct compile_dmajor_succ.
-    erewrite MixSemantics.mix_trace_fsim_match_val_compose.
-    Focus 2. eapply fsim_emajor_match_val; eauto.
-
-    instantiate (1 := eq).
-    split; intros; try break_exists; try break_and.
-    congruence. eauto.
-
-    erewrite Emajortodmajor.match_val_eq.
-    reflexivity.
-  Qed.
-    
-End FSIMdmajor.
-
-Section FSIMdflatmajor.
-
-  Variable dfm : Dmajor.program.
-  Hypothesis TRANSF : transf_untyped_to_dflatmajor M u1p = OK dfm.
-  
-  Lemma compile_dflatmajor_succ :
-    { c | transf_untyped_to_dmajor M u1p = Some c }.
-  Proof.
-    unfold transf_untyped_to_dflatmajor in TRANSF. break_result_chain. eauto.
-  Qed.
-  
-  Definition fsim_dflatmajor : MixSemantics.mix_forward_simulation (Untyped1.semantics u1p) (Dflatmajor.semantics dfm).
-    destruct compile_dflatmajor_succ.
-    eapply MixSemantics.compose_mix_trace_forward_simulation;
-      try eapply fsim_dmajor; eauto;
-        try eapply Dmajortodflatmajor.fsim; eauto.
-    unfold transf_untyped_to_dflatmajor in *;
-      unfold transf_untyped_to_dmajor in *;
-      break_result_chain;
-      try inv e;
-      congruence.
-  Defined.
-
-  Lemma fsim_dflatmajor_match_val :
-    forall x y,
-      MixSemantics.fsim_match_val _ _ fsim_dflatmajor x y <-> match_vals3 x y.
-  Proof.
-    intros. unfold fsim_dflatmajor.
-    destruct compile_dflatmajor_succ.
-    erewrite MixSemantics.mix_trace_fsim_match_val_compose.
-    Focus 2. eapply fsim_dmajor_match_val; eauto.
-
-    instantiate (1 := eq).
-    split; intros; try break_exists; try break_and.
-    congruence. eauto.
-
-    erewrite Dmajortodflatmajor.match_val_eq.
-    reflexivity.
-  Qed.
-    
-End FSIMdflatmajor.
-
-Section FSIMcmajor.
-
-  Variable Cm : Cmajor.program.
-  Hypothesis TRANSF : transf_untyped_to_cmajor M u1p = OK Cm.
-  
-  Lemma compile_cmajor_succ :
-    { c | transf_untyped_to_dflatmajor M u1p = Some c }.
-  Proof.
-    unfold transf_untyped_to_cmajor in TRANSF. break_result_chain. eauto.
-  Qed.
-  
-  Definition fsim_cmajor : MixSemantics.mix_forward_simulation (Untyped1.semantics u1p) (Cmajor.semantics Cm).
-    destruct compile_cmajor_succ.
-    eapply MixSemantics.compose_mix_trace_forward_simulation;
-      try eapply fsim_dflatmajor; eauto;
-        try eapply Dflatmajortocmajor.fsim; eauto.
-    unfold transf_untyped_to_cmajor in *;
-      unfold transf_untyped_to_dflatmajor in *;
-      break_result_chain;
-      try inv e;
-      congruence.
-  Defined.
-
-  Lemma fsim_cmajor_match_val :
-    forall x y,
-      MixSemantics.fsim_match_val _ _ fsim_cmajor x y <-> match_vals3 x y.
-  Proof.
-    intros. unfold fsim_cmajor.
-    destruct compile_cmajor_succ.
-    erewrite MixSemantics.mix_trace_fsim_match_val_compose.
-    Focus 2. eapply fsim_dflatmajor_match_val; eauto.
-
-    instantiate (1 := eq).
-    split; intros; try break_exists; try break_and.
-    congruence. eauto.
-
-    erewrite Dflatmajortocmajor.match_val_eq.
-    reflexivity.
-  Qed.
-    
-End FSIMcmajor.
 
 
 Section FSIMcminor.
 
-  Variable cm : Cminor.program.
-  Hypothesis TRANSF : transf_untyped_to_cminor M u1p = OK cm.
-  
-  Lemma compile_cminor_succ :
-    { c | transf_untyped_to_cmajor M u1p = Some c }.
-  Proof.
-    unfold transf_untyped_to_cminor in TRANSF. break_result_chain. eauto.
+  Variable a : Untyped1.prog_type.
+  Variable b : Cmajor.Cminor_program.
+  Variable M : MatchValues.id_map.
+  Hypothesis TRANSF : transf_untyped_to_cminor M a = OK b.
+
+  Definition fsim :
+        FullSemantics.forward_simulation
+        (Semantics.lift (Untyped1.semantics a)) (Cmajor.Cminor_semantics b) M.
+    unfold transf_untyped_to_cminor in *. break_result_chain.
+
+    eapply FullSemantics.compose_forward_simulation.
+      { eapply UntypedCompCombined.fsim; eauto. }
+    eapply FullSemantics.compose_forward_simulation.
+      { eapply ElimFuncCompCombined.fsim; eauto. }
+    eapply FullSemantics.compose_forward_simulation.
+      { eapply StackCompCombined.fsim; eauto. }
+    eapply FullSemantics.compose_forward_simulation.
+      { eapply LocalsCompCombined.fsim; eauto. }
+    eapply FullSemantics.compose_forward_simulation.
+      { eapply FlatCompCombined.fsim; eauto. }
+
+    eapply FullSemantics.compose_forward_simulation.
+      { eapply FmajorComp.fsim; eauto. }
+
+    eapply FullSemantics.compose_forward_simulation.
+      { eapply Fmajortofflatmajor.fsim; eauto. }
+    eapply FullSemantics.compose_forward_simulation.
+      { eapply Fflatmajortoemajor.fsim; eauto. }
+    eapply FullSemantics.compose_forward_simulation.
+      { eapply Emajortodmajor.fsim; eauto. }
+    eapply FullSemantics.compose_forward_simulation.
+      { eapply Dmajortodflatmajor.fsim; eauto. }
+    eapply FullSemantics.compose_forward_simulation.
+      { eapply Dflatmajortocmajor.fsim; eauto. }
+
+    eapply Cmajortominor.fsim; eauto.
   Qed.
-  
-  Definition fsim_cminor : MixSemantics.mix_forward_simulation (Untyped1.semantics u1p) (Cminor_semantics cm).
-    destruct compile_cminor_succ.
-    eapply MixSemantics.compose_mix_trace_forward_simulation;
-      try eapply fsim_cmajor; eauto;
-        try eapply Cmajortominor.fsim; eauto.
-    unfold transf_untyped_to_cminor in *;
-      unfold transf_untyped_to_cmajor in *;
-      break_result_chain;
-      try inv e.
-    rewrite OeufCompcertCompiler.print_identity in *.
-      congruence.
-  Defined.
 
-  Lemma fsim_cminor_match_val :
-    forall x y,
-      MixSemantics.fsim_match_val _ _ fsim_cminor x y <-> match_vals3 x y.
-  Proof.
-    intros. unfold fsim_cminor.
-    destruct compile_cminor_succ.
-    erewrite MixSemantics.mix_trace_fsim_match_val_compose.
-    Focus 2. eapply fsim_cmajor_match_val; eauto.
-
-    instantiate (1 := eq).
-    split; intros; try break_exists; try break_and.
-    congruence. eauto.
-
-    erewrite Cmajortominor.match_val_eq.
-    reflexivity.
-  Qed.
-    
 End FSIMcminor.
 
-End IDMap.
-End MATCH_VAL_INDICES.
-
-
-Ltac unfold_all_transf H :=
-    unfold transf_untyped_to_cminor in H;
-    unfold transf_untyped_to_cmajor in H;
-    unfold transf_untyped_to_dflatmajor in H;
-    unfold transf_untyped_to_dmajor in H;
-    unfold transf_untyped_to_emajor in H;
-    unfold transf_untyped_to_fflatmajor in H;
-    unfold transf_untyped_to_fmajor in H;
-    unfold transf_untyped_to_flat in H;
-    unfold transf_untyped_to_locals in H;
-    unfold transf_untyped_to_stack in H;
-    unfold transf_untyped_to_value_flag in H;
-    unfold transf_untyped_to_self_close in H;
-    unfold transf_untyped_to_switched in H;
-    unfold transf_untyped_to_elim_func3 in H;
-    unfold transf_untyped_to_elim_func2 in H;
-    unfold transf_untyped_to_elim_func in H;
-    unfold transf_untyped_to_tagged_numbered in H;
-    unfold transf_untyped_to_tagged in H.
-  
-
-Section Simulation.
-
-  
-  Variable prog : Untyped1.prog_type.
-  Variable tprog : Cminor.program.
-  Variable M : MatchValues.id_map.
-  Hypothesis TRANSF : transf_untyped_to_cminor M prog = OK tprog.
-
-
-  Lemma to_elim_func :
-    { pair | transf_untyped_to_elim_func prog = OK (fst pair) /\ ElimFuncComp2.compile_cu (fst pair) = Some (snd pair)}.
-  Proof.
-    unfold transf_untyped_to_cminor in TRANSF;
-    unfold transf_untyped_to_cmajor in TRANSF;
-    unfold transf_untyped_to_dflatmajor in TRANSF;
-    unfold transf_untyped_to_dmajor in TRANSF;
-    unfold transf_untyped_to_emajor in TRANSF;
-    unfold transf_untyped_to_fflatmajor in TRANSF;
-    unfold transf_untyped_to_fmajor in TRANSF;
-    unfold transf_untyped_to_flat in TRANSF;
-    unfold transf_untyped_to_locals in TRANSF;
-    unfold transf_untyped_to_stack in TRANSF;
-    unfold transf_untyped_to_value_flag in TRANSF;
-    unfold transf_untyped_to_self_close in TRANSF;
-    unfold transf_untyped_to_switched in TRANSF;
-    unfold transf_untyped_to_elim_func3 in TRANSF;
-    unfold transf_untyped_to_elim_func2 in TRANSF.
-    break_result_chain.
-    exists (p14, p13).
-    eauto.
-  Defined.
-
-  Definition efp : ElimFunc.prog_type.
-    destruct to_elim_func. exact (fst x).
-  Defined.
-
-  Definition efp2 : ElimFunc2.prog_type.
-    destruct to_elim_func. exact (snd x).
-  Defined.
-
-  (* In this theorem we grab all of the things we need from all of the passes *)
-  Theorem Oeuf_forward_simulation :
-      mix_forward_simulation (@Untyped1.semantics prog) (Cminor_semantics tprog).
-  Proof.
-    destruct to_elim_func.
-    destruct x. simpl in *. break_and. eapply fsim_cminor; eauto.
-  Defined.    
-  
-  Definition oeuf_match_vals (hv : HighestValues.value) (v : value) : Prop.
-    eapply match_vals3; try assumption.
-    exact efp. exact efp2.
-  Defined.
-    
-  Lemma Oeuf_fsim_match_val :
-    forall x y,
-      MixSemantics.fsim_match_val _ _ Oeuf_forward_simulation x y <-> oeuf_match_vals x y.
-  Proof.
-    intros. unfold Oeuf_forward_simulation.
-    repeat break_let.
-    erewrite fsim_cminor_match_val.
-    unfold oeuf_match_vals. 
-    unfold efp. unfold efp2. rewrite Heqs. simpl. reflexivity.
-  Qed.
-
-End Simulation.
 
 Section OeufSimulation.
     Variable P1 : CompilationUnit.compilation_unit.
     Let G := CompilationUnit.types P1.
     Let g := CompilationUnit.exprs P1.
 
-    Variable P3 : Cminor.program.
+    Variable P3 : Cminor_program.
     Let L3 := Cminor_semantics P3.
 
     Variable M : MatchValues.id_map.
-    
-    Hypothesis TRANSF : transf_oeuf_to_cminor M P1 = OK P3.
 
-    Definition UTTRANSF :
-      { ut | transf_oeuf_to_untyped1 P1 = OK ut }.
+    Hypothesis TRANSF13 : transf_oeuf_to_cminor M P1 = OK P3.
+
+
+    Definition P2_TRANSF :
+      { P2 |
+              transf_oeuf_to_untyped1 P1 = OK P2 /\
+              transf_untyped_to_cminor M P2 = OK P3 }.
     Proof.
       unfold transf_oeuf_to_cminor in *. break_result_chain.
       eauto.
     Defined.
 
-    Definition ut : Untyped1.prog_type := proj1_sig UTTRANSF.
-    Definition ut_trans := proj2_sig UTTRANSF.
+    Definition P2 : Untyped1.prog_type := proj1_sig P2_TRANSF.
+    Let L2 := Untyped1.semantics P2.
+    Let L2' := Semantics.lift L2.
 
-    Lemma trans_ut :
-      transf_untyped_to_cminor M ut = OK P3.
-    Proof.
-      copy TRANSF.
-      unfold transf_oeuf_to_cminor in H.
-      rewrite ut_trans in H.
-      break_result_chain. fold ut in H. assumption.
+    Definition TRANSF12 : transf_oeuf_to_untyped1 P1 = OK P2 := proj1 (proj2_sig P2_TRANSF).
+    Definition TRANSF23 : transf_untyped_to_cminor M P2 = OK P3 := proj2 (proj2_sig P2_TRANSF).
+
+    Lemma S23 : FullSemantics.forward_simulation L2' L3 M.
+    eapply fsim. exact TRANSF23.
     Qed.
-    
-    Definition EFTRANSF :
-      { pair | transf_untyped_to_elim_func ut = OK (fst pair) /\ ElimFuncComp2.compile_cu (fst pair) = Some (snd pair)}.
-    Proof.
-      copy TRANSF.
-      unfold transf_oeuf_to_cminor in H.
-      rewrite ut_trans in H.
-      unfold transf_untyped_to_cminor in H;
-        unfold transf_untyped_to_cmajor in H;
-        unfold transf_untyped_to_dflatmajor in H;
-        unfold transf_untyped_to_dmajor in H;
-        unfold transf_untyped_to_emajor in H;
-        unfold transf_untyped_to_fflatmajor in H;
-        unfold transf_untyped_to_fmajor in H;
-        unfold transf_untyped_to_flat in H;
-        unfold transf_untyped_to_locals in H;
-        unfold transf_untyped_to_stack in H;
-        unfold transf_untyped_to_value_flag in H;
-        unfold transf_untyped_to_self_close in H;
-        unfold transf_untyped_to_switched in H;
-        unfold transf_untyped_to_elim_func3 in H;
-        unfold transf_untyped_to_elim_func2 in H.
-      break_result_chain.
-      fold ut in Heqr14.
-      exists (p14, p13).
-      eauto.
-    Defined.
-    
-    Definition EFP : ElimFunc.prog_type := fst (proj1_sig EFTRANSF).
-    Definition EFP2 : ElimFunc2.prog_type := snd (proj1_sig EFTRANSF).
 
 
-    (*
-    
-    Definition FLATTRANSF :
-      { flat | transf_untyped_to_flat ut = OK flat }.
-    Proof.
-      copy TRANSF. unfold transf_oeuf_to_cminor in H.
-      rewrite ut_trans in H. fold ut in H.
-      unfold transf_untyped_to_cminor in H;
-        unfold transf_untyped_to_cmajor in H;
-        unfold transf_untyped_to_dflatmajor in H;
-        unfold transf_untyped_to_dmajor in H;
-        unfold transf_untyped_to_emajor in H;
-        unfold transf_untyped_to_fflatmajor in H;
-        unfold transf_untyped_to_fmajor in H.
-      break_result_chain.
-      eauto.
-    Defined.
+    Definition oeuf_index := FullSemantics.fsim_index S23.
+    Definition oeuf_order := FullSemantics.fsim_order S23.
+    Definition oeuf_order_wf := FullSemantics.fsim_order_wf S23.
+    Definition oeuf_match_states {rty} i (s1 : SourceLifted.state G rty) s3 :=
+        exists s2,
+            UntypedComp1.compile_state s1 = s2 /\
+            FullSemantics.fsim_match_states S23 i s2 s3.
+    Definition oeuf_match_val {ty} (v1 : SourceLifted.value G ty) v3 :=
+        exists v2,
+            UntypedComp1.compile_value v1 = v2 /\
+            FullSemantics.fsim_match_val S23 v2 v3.
 
-    Definition FLAT : FlatIntTag.prog_type := proj1_sig FLATTRANSF.
-    Definition flat_transf := proj2_sig FLATTRANSF.
-
-    Definition BLS: 
-      { M | FmajorComp.build_id_list FLAT = Some M }.
-    Proof.
-      copy TRANSF. unfold transf_oeuf_to_cminor in H.
-      rewrite ut_trans in H. fold ut in H.
-      unfold transf_untyped_to_cminor in H;
-        unfold transf_untyped_to_cmajor in H;
-        unfold transf_untyped_to_dflatmajor in H;
-        unfold transf_untyped_to_dmajor in H;
-        unfold transf_untyped_to_emajor in H;
-        unfold transf_untyped_to_fflatmajor in H;
-        unfold transf_untyped_to_fmajor in H.
-      break_result_chain.
-      unfold FmajorComp.compile_cu_intern in *.
-      repeat break_bind_option. rewrite flat_transf in Heqr6. fold FLAT in Heqr6.
-      invc Heqr6.
-      eauto.
-    Defined.
-
-    Definition MMM := proj1_sig BLS.
-*)    
-
-    Definition oeuf_index :=
-        sl_index ut L3 (Oeuf_forward_simulation ut P3 M trans_ut).
-    Definition oeuf_order :=
-        sl_order ut L3 (Oeuf_forward_simulation ut P3 M trans_ut).
-    Definition oeuf_match_states {rty} :=
-        @sl_match_states P1 ut L3 (Oeuf_forward_simulation ut P3 M trans_ut) rty.
-    Definition oeuf_match_values {ty} :=
-        @sl_match_values P1 ut L3 (Oeuf_forward_simulation ut P3 M trans_ut) ty.
-
-    Definition match_values {ty A B l M} (slv : SourceLifted.value (types P1) ty) (hv : value) : Prop :=
-      exists hstv hrv hrv' hv0,
-        MatchValues.compile_highest slv = hstv /\
-        TaggedComp.I_value hstv hrv /\
-        ElimFuncComp2.match_values A B l hrv hrv' /\
-        FlatIntTagComp.I_value hrv' hv0 /\
-        FmajorComp.I_value M hv0 hv.
-    
-    Lemma match_val_eq :
-      forall {ty} x y,
-        @oeuf_match_values ty x y <-> @match_values ty (fst EFP) (fst EFP2) (snd EFP) M x y.
-    Proof.
-      unfold oeuf_match_values. unfold sl_match_values.
-      unfold L3 in *.
-      intros.
-      split; intros.
-
-
-      break_exists.
-      break_and.
-      rewrite Oeuf_fsim_match_val in H0.
-      unfold match_values. unfold oeuf_match_vals in *.
-
-      inversion H0. repeat (break_exists); repeat break_and.
-
-      (* EFP and EFP2 *)
-      unfold efp in *. unfold efp2 in *. unfold EFP. unfold EFP2. destruct EFTRANSF.
-      destruct to_elim_func.
-      break_and. destruct x4. destruct x5.
-      destruct p. destruct p0. destruct p1. destruct p2.
-      unfold fst in *. unfold snd in *.
-      rewrite e in H5.
-      inversion H5. subst l l0.
-      rewrite e0 in H6. inversion H6.
-      subst l1 l2.
-      unfold proj1_sig.
-      do 4 eexists.
-      repeat (split; try eassumption).
-
-
-      inversion H.
-      repeat break_exists. repeat break_and.
-      exists x0. split; try assumption.
-      rewrite Oeuf_fsim_match_val.
-      unfold oeuf_match_vals.
-      unfold match_vals3.
-      unfold match_val_highest_high'.
-
-      unfold efp. unfold efp2. unfold EFP in *. unfold EFP2 in *. destruct EFTRANSF.
-      destruct to_elim_func.
-      break_and. destruct x4. destruct x5.
-      destruct p. destruct p0. destruct p1. destruct p2.
-      unfold fst in *. unfold snd in *.
-      unfold proj1_sig in *.
-      
-      rewrite e in H5.
-      inversion H5. subst l l0.
-      rewrite e0 in H6. inversion H6.
-      subst l1 l2.
-      do 3 eexists.
-      repeat (split; try eassumption).
-    Qed.
-    
     Theorem oeuf_match_callstate :
         forall tyA tyR
             (fv1 : SourceLifted.value G (SourceLifted.Arrow tyA tyR))
@@ -1271,33 +191,27 @@ Section OeufSimulation.
             (fv3 av3 : HighValues.value)
             (s3 : Cminor.state),
         cminor_is_callstate P3 fv3 av3 s3 ->
-        @match_values _ (fst EFP) (fst EFP2) (snd EFP) M fv1 fv3 ->
-        @match_values _ (fst EFP) (fst EFP2) (snd EFP) M av1 av3 ->
+        oeuf_match_val fv1 fv3 ->
+        oeuf_match_val av1 av3 ->
         exists s1 i,
             oeuf_match_states i s1 s3 /\
             SourceLifted.is_callstate g fv1 av1 s1.
-      intros.
-      rewrite <- match_val_eq in H0.
-      rewrite <- match_val_eq in H1.
-      eapply sl_match_callstate; try eassumption.
-      
-      eapply ut_trans.
-    Qed.
+    intros.
 
-    Theorem oeuf_match_final_states' :
-        forall ty i
-            (s1 : SourceLifted.state G ty)
-            (s3 : Cminor.state)
-            (v1 : SourceLifted.value G ty),
-        oeuf_match_states i s1 s3 ->
-        SourceLifted.final_state s1 v1 ->
-        exists v3,
-            cminor_final_state P3 s3 v3 /\
-            oeuf_match_values v1 v3.
-      intros.
-      
-      fwd eapply sl_match_final_states; try eassumption;
-        try eapply ut_trans.
+    unfold oeuf_match_val in *.  break_exists. break_and.
+
+    fwd eapply (FullSemantics.fsim_match_callstate S23); eauto.
+      do 2 break_exists. break_and.
+
+    fwd eapply (UntypedComp1.match_callstate) with (Bmeta := snd P2).
+      { eapply transf_oeuf_to_untyped1_genv. exact TRANSF12. }
+      { rewrite <- surjective_pairing. eauto. }
+      { eauto. }
+      { eauto. }
+      break_exists. break_and.
+
+    do 2 eexists. split; eauto.
+    eexists. split; eauto.
     Qed.
 
     Theorem oeuf_match_final_states :
@@ -1309,12 +223,26 @@ Section OeufSimulation.
         SourceLifted.final_state s1 v1 ->
         exists v3,
             cminor_final_state P3 s3 v3 /\
-            @match_values _ (fst EFP) (fst EFP2) (snd EFP) M v1 v3.
-    Proof.
-      intros.
-      edestruct oeuf_match_final_states'; try eassumption.
-      break_and. eexists. split. eassumption.
-      eapply match_val_eq. apply H2.
+            oeuf_match_val v1 v3.
+    intros.
+
+    unfold oeuf_match_states in *.  break_exists. break_and.
+
+    fwd eapply (UntypedComp1.match_final_state) with (Bmeta := snd P2).
+      { eapply transf_oeuf_to_untyped1_genv. exact TRANSF12. }
+      { eapply transf_oeuf_to_untyped1_meta_public. exact TRANSF12. }
+      { eapply transf_oeuf_to_untyped1_nfree. exact TRANSF12. }
+      { eapply transf_oeuf_to_untyped1_meta_len. exact TRANSF12. }
+      { eauto. }
+      { eauto. }
+    break_exists. break_and.
+      rewrite <- surjective_pairing in *.
+
+    fwd eapply (FullSemantics.fsim_match_final_states S23); eauto.
+      break_exists. break_and.
+
+    eexists. split; eauto.
+    eexists. eauto.
     Qed.
 
     Theorem oeuf_simulation :
@@ -1323,20 +251,56 @@ Section OeufSimulation.
         forall i s3,
         oeuf_match_states i s1 s3 ->
         exists i', exists s3',
-            ((TraceSemantics.plus Cminor.step (Genv.globalenv P3)
+            ((FullSemantics.plus Cminor.step (Genv.globalenv P3)
                     s3 Events.E0 s3') \/
-                (TraceSemantics.star Cminor.step (Genv.globalenv P3)
+                (FullSemantics.star Cminor.step (Genv.globalenv P3)
                         s3 Events.E0 s3' /\
                     oeuf_order i' i)) /\
             oeuf_match_states i' s1' s3'.
     intros.
-    eapply sl_simulation; try eassumption.
-    eapply ut_trans.
+
+    unfold oeuf_match_states in *.  break_exists. break_and.
+
+    fwd eapply (UntypedComp1.I_sim).
+      { eapply transf_oeuf_to_untyped1_genv. exact TRANSF12. }
+      { eauto. }
+      { eauto. }
+    break_exists. break_and.
+
+    fwd eapply (FullSemantics.fsim_simulation S23); eauto.
+      { simpl. split; eauto. }
+    break_exists. break_and.
+    break_or; break_and.
+    all: do 2 eexists; split; eauto.
     Qed.
-    
+
+    Lemma oeuf_val_level_le :
+        forall {ty},
+        value_level_le_indexed (VlSource G ty) VlHigh.
+    intros. simpl. auto.
+    Qed.
+
+    Theorem oeuf_match_val_canon :
+        forall {ty} (v1 : SourceLifted.value G ty) (v3 : HighValues.value),
+        oeuf_match_val v1 v3 <->
+        value_match_indexed M (VlSource G ty) VlHigh v1 v3.
+    intros. split; intro HH.
+
+    - destruct HH as (v2 & ? & ?).
+      eapply value_match_indexed_compose.
+      2: eapply (FullSemantics.fsim_match_val_canon S23); eassumption.
+      simpl. auto.
+
+    - eapply value_match_indexed_decompose with (vl2 := VlHighest) in HH; [ | simpl; eauto.. ].
+        break_exists. break_and.
+      eexists. split; eauto.
+      eapply (FullSemantics.fsim_match_val_canon S23). eassumption.
+    Qed.
+
+
     Theorem oeuf_star_simulation :
         forall rty (s1 s1' : SourceLifted.state G rty),
-          Semantics.star _ _ SourceLifted.sstep g s1 s1' ->
+          Semantics.star SourceLifted.sstep g s1 s1' ->
         forall i s3,
           oeuf_match_states i s1 s3 ->
           exists i' s3',
@@ -1349,19 +313,21 @@ Section OeufSimulation.
       eapply oeuf_simulation in H.
       Focus 2. eassumption.
       repeat break_exists. repeat break_and.
-      break_or. eapply TraceSemantics.plus_star in H.
+      break_or. eapply FullSemantics.plus_star in H.
       eapply IHstar in H2. repeat break_exists; repeat break_and.
       eexists; eexists; split.
-      eapply TraceSemantics.star_trans. eassumption.
+      eapply FullSemantics.star_trans. eassumption.
       eassumption. reflexivity.
       eassumption.
       break_and.
       eapply IHstar in H2. repeat break_exists; repeat break_and.
       eexists; eexists; split.
-      eapply TraceSemantics.star_trans. eassumption.
+      eapply FullSemantics.star_trans. eassumption.
       eassumption. reflexivity.
       eassumption.
     Qed.
+
+
 
 (* Let s ′ be a Cminor callstate, representing an application of the
 Cminor closure value f ′ to the Cminor value a′. Suppose there
@@ -1376,18 +342,18 @@ Require Import SourceLiftedProofs.
 Inductive value_match (ty : type) (gv : type_denote ty) (hv : HighValues.value) : Prop :=
 | mv :
     forall (slv : SourceLifted.value G ty),
-      @match_values _ (fst EFP) (fst EFP2) (snd EFP) M slv hv ->
       value_denote (genv_denote g) slv = gv ->
+      oeuf_match_val slv hv ->
       value_match ty gv hv.
 
 Axiom sourcelifted_termination :
   forall G rty (st : SourceLifted.state G rty) (g : SourceLifted.genv G),
   exists v,
-    Semantics.star _ _ (SourceLifted.sstep) g st (SourceLifted.Stop v).
+    Semantics.star (SourceLifted.sstep) g st (SourceLifted.Stop v).
 
 Lemma star_sstep_denote :
   forall G (g : SourceLifted.genv G) rty (s1 s2: SourceLifted.state G rty),
-    Semantics.star _ _ SourceLifted.sstep g s1 s2 ->
+    Semantics.star SourceLifted.sstep g s1 s2 ->
     state_denote (genv_denote g) s1 = state_denote (genv_denote g) s2.
 Proof.
   induction 1; intros.
@@ -1408,33 +374,26 @@ Theorem oeuf_spec :
       TraceSemantics.star Cminor.step (Genv.globalenv P3) cmst E0 cmst' /\
       cminor_final_state P3 cmst' rhv /\
       value_match tyR (fv av) rhv.
-Proof.
-  intros.
-  inversion H0. inversion H1.
-  eapply oeuf_match_callstate in H; eauto.
-  repeat (break_exists; break_and).
-  pose proof (sourcelifted_termination _ _ x g).
-  break_exists.
-  pose proof H7 as Hstar.
-  eapply oeuf_star_simulation in H7; try eassumption.
-  repeat (break_exists; break_and).
-  assert (SourceLifted.final_state (Stop x1) x1) by
-      constructor.
-  copy H9.
-  eapply oeuf_match_final_states in H9; try eassumption.
-  repeat (break_exists; break_and).
-  exists x3. exists x4.
-  split; try eassumption.
-  split; try eassumption.
-  econstructor. eassumption.
-  eapply denote_callstate in H6.
-  eapply denote_finalstate in H10.
-  instantiate (1 := g) in H10.
-  eapply star_sstep_denote in Hstar.
+intros.
+do 2 on >value_match, invc.
+
+fwd eapply oeuf_match_callstate; eauto.
+  break_exists. break_and.
+fwd eapply sourcelifted_termination with (st := x) as HH.
+  destruct HH as (v & ?).
+assert (SourceLifted.final_state (Stop v) v) by constructor.
+fwd eapply oeuf_star_simulation; eauto.
+  break_exists. break_and.
+fwd eapply oeuf_match_final_states; eauto.
+  break_exists. break_and.
+
+do 2 eexists. split; [|split]; eauto.
+- econstructor; eauto.
+  fwd eapply denote_callstate; eauto.
+  fwd eapply denote_finalstate with (g := g); eauto.
+  fwd eapply star_sstep_denote; eauto.
+  unfold G in *. (* fix implicits *)
   congruence.
 Qed.
-            
-            
-
     
 End OeufSimulation.
