src/Semantics.v
@@ -13,30 +13,26 @@ Require Import StructTact.StructTactics.
 Require Import StructTact.Util.
 
 Require Import EricTact.
+Require Import StuartTact.
 
 Require Import AllValues.
+Require Import MatchValues.
+
+Require FullSemantics.
+
+Set Default Timeout 15.
+Set Implicit Arguments.
+
 
 Section CLOSURES.
 
 Variable genv: Type.
 Variable state: Type.
 
-(** A one-step transition relation has the following signature.
-  It is parameterized by a global environment, which does not
-  change during the transition.  It relates the initial state
-  of the transition with its final state.  The [trace] parameter
-  captures the observable events possibly generated during the
-  transition. *)
-
 Variable step: genv -> state -> state -> Prop.
-
-(** No transitions: stuck state *)
 
 Definition nostep (ge: genv) (s: state) : Prop :=
   forall s', ~(step ge s s').
-
-(** Zero, one or several transitions.  Also known as Kleene closure,
-    or reflexive transitive closure. *)
 
 Inductive star (ge: genv): state -> state -> Prop :=
   | star_refl: forall s,
@@ -45,428 +41,33 @@ Inductive star (ge: genv): state -> state -> Prop :=
       step ge s1 s2 -> star ge s2 s3 -> 
       star ge s1 s3.
 
-Lemma star_one:
-  forall ge s1 s2, step ge s1 s2 -> star ge s1 s2.
-Proof.
-  intros. eapply star_step; eauto. apply star_refl. 
-Qed.
-
-Lemma star_two:
-  forall ge s1 s2 s3,
-  step ge s1 s2 -> step ge s2 s3 ->
-  star ge s1 s3.
-Proof.
-  intros. eapply star_step; eauto. apply star_one; auto.
-Qed.
-
-(* 
-
-Lemma star_three:
-  forall ge s1 t1 s2 t2 s3 t3 s4 t,
-  step ge s1 t1 s2 -> step ge s2 t2 s3 -> step ge s3 t3 s4 -> t = t1 ** t2 ** t3 ->
-  star ge s1 t s4.
-Proof.
-  intros. eapply star_step; eauto. eapply star_two; eauto.
-Qed.
-
-Lemma star_four:
-  forall ge s1 t1 s2 t2 s3 t3 s4 t4 s5 t,
-  step ge s1 t1 s2 -> step ge s2 t2 s3 ->
-  step ge s3 t3 s4 -> step ge s4 t4 s5 -> t = t1 ** t2 ** t3 ** t4 ->
-  star ge s1 t s5.
-Proof.
-  intros. eapply star_step; eauto. eapply star_three; eauto.
-Qed.
-
-*)
-
-Lemma star_trans:
-  forall ge s1 s2, star ge s1 s2 ->
-  forall s3, star ge s2 s3 -> star ge s1 s3.
-Proof.
-  induction 1; intros; eauto.
-  eapply star_step; eauto. 
-Qed.
-
-Lemma star_left:
-  forall ge s1 s2 s3,
-  step ge s1 s2 -> star ge s2 s3 -> 
-  star ge s1 s3.
-Proof star_step.
-
-Lemma star_right:
-  forall ge s1 s2 s3,
-  star ge s1 s2 -> step ge s2 s3 -> 
-  star ge s1 s3.
-Proof.
-  intros. eapply star_trans. eauto. apply star_one. eauto. 
-Qed.
-
-(* 
-Lemma star_E0_ind:
-  forall ge (P: state -> state -> Prop),
-  (forall s, P s s) ->
-  (forall s1 s2 s3, step ge s1 E0 s2 -> P s2 s3 -> P s1 s3) ->
-  forall s1 s2, star ge s1 E0 s2 -> P s1 s2.
-Proof.
-  intros ge P BASE REC.
-  assert (forall s1 t s2, star ge s1 t s2 -> t = E0 -> P s1 s2).
-    induction 1; intros; subst.
-    auto.
-    destruct (Eapp_E0_inv _ _ H2). subst. eauto.
-  eauto.
-Qed.
- *)
-
-(** One or several transitions.  Also known as the transitive closure. *)
-
 Inductive plus (ge: genv): state -> state -> Prop :=
   | plus_left: forall s1 s2 s3,
       step ge s1 s2 -> star ge s2 s3 -> 
       plus ge s1 s3.
 
-Lemma plus_one:
-  forall ge s1 s2,
-  step ge s1 s2 -> plus ge s1 s2.
-Proof.
-  intros. econstructor; eauto. apply star_refl. 
+Section CLOSURES_LIFT.
+
+Variable tstep : genv -> state -> trace -> state -> Prop.
+
+Hypothesis lift_step : forall ge s s', step ge s s' -> tstep ge s E0 s'.
+
+Lemma lift_star : forall ge s s', star ge s s' -> FullSemantics.star tstep ge s E0 s'.
+induction 1; simpl in *.
+- econstructor.
+- econstructor; eauto.
 Qed.
 
-(*
-Lemma plus_two:
-  forall ge s1 t1 s2 t2 s3 t,
-  step ge s1 t1 s2 -> step ge s2 t2 s3 -> t = t1 ** t2 ->
-  plus ge s1 t s3.
-Proof.
-  intros. eapply plus_left; eauto. apply star_one; auto.
+Lemma lift_plus : forall ge s s', plus ge s s' -> FullSemantics.plus tstep ge s E0 s'.
+induction 1; simpl in *.
+- econstructor; eauto using lift_star.
 Qed.
 
-Lemma plus_three:
-  forall ge s1 t1 s2 t2 s3 t3 s4 t,
-  step ge s1 t1 s2 -> step ge s2 t2 s3 -> step ge s3 t3 s4 -> t = t1 ** t2 ** t3 ->
-  plus ge s1 t s4.
-Proof.
-  intros. eapply plus_left; eauto. eapply star_two; eauto.
-Qed.
+End CLOSURES_LIFT.
 
-Lemma plus_four:
-  forall ge s1 t1 s2 t2 s3 t3 s4 t4 s5 t,
-  step ge s1 t1 s2 -> step ge s2 t2 s3 ->
-  step ge s3 t3 s4 -> step ge s4 t4 s5 -> t = t1 ** t2 ** t3 ** t4 ->
-  plus ge s1 t s5.
-Proof.
-  intros. eapply plus_left; eauto. eapply star_three; eauto.
-Qed.
-*)
-
-
-Lemma plus_star:
-  forall ge s1 s2, plus ge s1 s2 -> star ge s1 s2.
-Proof.
-  intros. inversion H; subst.
-  eapply star_step; eauto.
-Qed.
-
-Lemma plus_right:
-  forall ge s1 s2 s3,
-  star ge s1 s2 -> step ge s2 s3 -> 
-  plus ge s1 s3.
-Proof.
-  intros. inversion H; subst. simpl. apply plus_one. auto.
-  eapply plus_left; eauto.
-  eapply star_right; eauto.
-Qed.
-
-Lemma plus_left':
-  forall ge s1 s2 s3,
-  step ge s1 s2 -> plus ge s2 s3 -> 
-  plus ge s1 s3.
-Proof.
-  intros. eapply plus_left; eauto. apply plus_star; auto.
-Qed.
-
-Lemma plus_right':
-  forall ge s1 s2 s3,
-  plus ge s1 s2 -> step ge s2 s3 -> 
-  plus ge s1 s3.
-Proof.
-  intros. eapply plus_right; eauto. apply plus_star; auto.
-Qed.
-
-Lemma plus_star_trans:
-  forall ge s1 s2 s3,
-  plus ge s1 s2 -> star ge s2 s3  -> plus ge s1 s3.
-Proof.
-  intros. inversion H; subst.
-  econstructor; eauto. eapply star_trans; eauto.
-Qed.
-
-Lemma star_plus_trans:
-  forall ge s1 s2 s3,
-  star ge s1 s2 -> plus ge s2 s3 -> plus ge s1 s3.
-Proof.
-  intros. inversion H; subst.
-  simpl; auto.
-  econstructor. eauto. eapply star_trans. eauto.
-  apply plus_star. eauto. 
-Qed.
-
-Lemma plus_trans:
-  forall ge s1 s2 s3,
-  plus ge s1 s2 -> plus ge s2 s3 -> plus ge s1 s3.
-Proof.
-  intros. eapply plus_star_trans. eauto. apply plus_star. eauto. 
-Qed.
-
-Lemma plus_inv:
-  forall ge s1 s2,
-  plus ge s1 s2 ->
-  step ge s1 s2 \/ exists s', step ge s1 s' /\ plus ge s' s2.
-Proof.
-  intros. inversion H; subst. inversion H1; subst.
-  left. auto.
-  right. exists s3; split. auto.
-  econstructor; eauto.
-Qed.
-
-Lemma star_inv:
-  forall ge s1 s2,
-  star ge s1 s2 ->
-  s2 = s1 \/ plus ge s1 s2.
-Proof.
-  intros. inv H. left; auto. right; econstructor; eauto.
-Qed.
-
-Lemma plus_ind2:
-  forall ge (P: state -> state -> Prop),
-  (forall s1 s2, step ge s1 s2 -> P s1 s2) ->
-  (forall s1 s2 s3,
-   step ge s1 s2 -> plus ge s2 s3 -> P s2 s3 -> 
-   P s1 s3) ->
-  forall s1 s2, plus ge s1 s2 -> P s1 s2.
-Proof.
-  intros ge P BASE IND.
-  assert (forall s1 s2, star ge s1 s2 ->
-         forall s0, step ge s0 s1 ->
-         P s0 s2).
-  induction 1; intros.
-  apply BASE; auto.
-  eapply IND. eauto. econstructor; eauto. eapply IHstar; eauto. auto.
-  intros. inv H0. eauto.
-Qed.
-
-(*
-Lemma plus_E0_ind:
-  forall ge (P: state -> state -> Prop),
-  (forall s1 s2 s3, step ge s1 E0 s2 -> star ge s2 E0 s3 -> P s1 s3) ->
-  forall s1 s2, plus ge s1 E0 s2 -> P s1 s2.
-Proof.
-  intros. inv H0. exploit Eapp_E0_inv; eauto. intros [A B]; subst. eauto.
-Qed.
-*)
-(** Counted sequences of transitions *)
-
-
-
-Inductive starN (ge: genv): nat -> state -> state -> Prop :=
-  | starN_refl: forall s,
-      starN ge O s s
-  | starN_step: forall n s s' s'',
-      step ge s s' -> starN ge n s' s'' -> 
-      starN ge (S n) s s''.
-
-Remark starN_star:
-  forall ge n s s', starN ge n s s' -> star ge s s'.
-Proof.
-  induction 1; econstructor; eauto.
-Qed.
-
-Remark star_starN:
-  forall ge s s', star ge s s' -> exists n, starN ge n s s'.
-Proof.
-  induction 1.
-  exists O; constructor.
-  destruct IHstar as [n P]. exists (S n); econstructor; eauto.
-Qed.
- 
-(** Infinitely many transitions *)
-
-(*
-CoInductive forever (ge: genv): state -> traceinf -> Prop :=
-  | forever_intro: forall s1 t s2 T,
-      step ge s1 t s2 -> forever ge s2 T ->
-      forever ge s1 (t *** T).
-
-Lemma star_forever:
-  forall ge s1 t s2, star ge s1 t s2 ->
-  forall T, forever ge s2 T ->
-  forever ge s1 (t *** T).
-Proof.
-  induction 1; intros. simpl. auto.
-  subst t. rewrite Eappinf_assoc.
-  econstructor; eauto.
-Qed.
-*)
-(** An alternate, equivalent definition of [forever] that is useful
-    for coinductive reasoning. *)
-(*
-Variable A: Type.
-Variable order: A -> A -> Prop.
-
-CoInductive forever_N (ge: genv) : A -> state -> traceinf -> Prop :=
-  | forever_N_star: forall s1 t s2 a1 a2 T1 T2,
-      star ge s1 t s2 ->
-      order a2 a1 ->
-      forever_N ge a2 s2 T2 ->
-      T1 = t *** T2 ->
-      forever_N ge a1 s1 T1
-  | forever_N_plus: forall s1 t s2 a1 a2 T1 T2,
-      plus ge s1 t s2 ->
-      forever_N ge a2 s2 T2 ->
-      T1 = t *** T2 ->
-      forever_N ge a1 s1 T1.
-
-Hypothesis order_wf: well_founded order.
-
-Lemma forever_N_inv:
-  forall ge a s T,
-  forever_N ge a s T ->
-  exists t, exists s', exists a', exists T',
-  step ge s t s' /\ forever_N ge a' s' T' /\ T = t *** T'.
-Proof.
-  intros ge a0. pattern a0. apply (well_founded_ind order_wf).
-  intros. inv H0.
-  (* star case *)
-  inv H1.
-  (* no transition *)
-  change (E0 *** T2) with T2. apply H with a2. auto. auto.
-  (* at least one transition *)
-  exists t1; exists s0; exists x; exists (t2 *** T2).
-  split. auto. split. eapply forever_N_star; eauto.
-  apply Eappinf_assoc.
-  (* plus case *)
-  inv H1.
-  exists t1; exists s0; exists a2; exists (t2 *** T2).
-  split. auto.
-  split. inv H3. auto.
-  eapply forever_N_plus. econstructor; eauto. eauto. auto.
-  apply Eappinf_assoc.
-Qed.
-
-Lemma forever_N_forever:
-  forall ge a s T, forever_N ge a s T -> forever ge s T.
-Proof.
-  cofix COINDHYP; intros.
-  destruct (forever_N_inv H) as [t [s' [a' [T' [P [Q R]]]]]].
-  rewrite R. apply forever_intro with s'. auto.
-  apply COINDHYP with a'; auto.
-Qed.
-
-(** Yet another alternative definition of [forever]. *)
-
-CoInductive forever_plus (ge: genv) : state -> traceinf -> Prop :=
-  | forever_plus_intro: forall s1 t s2 T1 T2,
-      plus ge s1 t s2 ->
-      forever_plus ge s2 T2 ->
-      T1 = t *** T2 ->
-      forever_plus ge s1 T1.
-
-Lemma forever_plus_inv:
-  forall ge s T,
-  forever_plus ge s T ->
-  exists s', exists t, exists T',
-  step ge s t s' /\ forever_plus ge s' T' /\ T = t *** T'.
-Proof.
-  intros. inv H. inv H0. exists s0; exists t1; exists (t2 *** T2).
-  split. auto.
-  split. exploit star_inv; eauto. intros [[P Q] | R].
-    subst. simpl. auto. econstructor; eauto.
-  traceEq.
-Qed.
-
-Lemma forever_plus_forever:
-  forall ge s T, forever_plus ge s T -> forever ge s T.
-Proof.
-  cofix COINDHYP; intros.
-  destruct (forever_plus_inv H) as [s' [t [T' [P [Q R]]]]].
-  subst. econstructor; eauto.
-Qed.
-
-(** Infinitely many silent transitions *)
-
-CoInductive forever_silent (ge: genv): state -> Prop :=
-  | forever_silent_intro: forall s1 s2,
-      step ge s1 E0 s2 -> forever_silent ge s2 ->
-      forever_silent ge s1.
-
-(** An alternate definition. *)
-
-CoInductive forever_silent_N (ge: genv) : A -> state -> Prop :=
-  | forever_silent_N_star: forall s1 s2 a1 a2,
-      star ge s1 E0 s2 ->
-      order a2 a1 ->
-      forever_silent_N ge a2 s2 ->
-      forever_silent_N ge a1 s1
-  | forever_silent_N_plus: forall s1 s2 a1 a2,
-      plus ge s1 E0 s2 ->
-      forever_silent_N ge a2 s2 ->
-      forever_silent_N ge a1 s1.
-
-Lemma forever_silent_N_inv:
-  forall ge a s,
-  forever_silent_N ge a s ->
-  exists s', exists a',
-  step ge s E0 s' /\ forever_silent_N ge a' s'.
-Proof.
-  intros ge a0. pattern a0. apply (well_founded_ind order_wf).
-  intros. inv H0.
-  (* star case *)
-  inv H1.
-  (* no transition *)
-  apply H with a2. auto. auto.
-  (* at least one transition *)
-  exploit Eapp_E0_inv; eauto. intros [P Q]. subst.
-  exists s0; exists x.
-  split. auto. eapply forever_silent_N_star; eauto.
-  (* plus case *)
-  inv H1. exploit Eapp_E0_inv; eauto. intros [P Q]. subst.
-  exists s0; exists a2.
-  split. auto. inv H3. auto.
-  eapply forever_silent_N_plus. econstructor; eauto. eauto.
-Qed.
-
-Lemma forever_silent_N_forever:
-  forall ge a s, forever_silent_N ge a s -> forever_silent ge s.
-Proof.
-  cofix COINDHYP; intros.
-  destruct (forever_silent_N_inv H) as [s' [a' [P Q]]].
-  apply forever_silent_intro with s'. auto.
-  apply COINDHYP with a'; auto.
-Qed.
-
-(** Infinitely many non-silent transitions *)
-
-CoInductive forever_reactive (ge: genv): state -> traceinf -> Prop :=
-  | forever_reactive_intro: forall s1 s2 t T,
-      star ge s1 t s2 -> t <> E0 -> forever_reactive ge s2 T ->
-      forever_reactive ge s1 (t *** T).
-
-Lemma star_forever_reactive:
-  forall ge s1 t s2 T,
-  star ge s1 t s2 -> forever_reactive ge s2 T ->
-  forever_reactive ge s1 (t *** T).
-Proof.
-  intros. inv H0. rewrite <- Eappinf_assoc. econstructor.
-  eapply star_trans; eauto.
-  red; intro. exploit Eapp_E0_inv; eauto. intros [P Q]. contradiction.
-  auto.
-Qed.
-*)
 End CLOSURES.
 
-(** * Transition semantics *)
 
-(** The general form of a transition semantics. *)
 
 Record semantics : Type := Semantics_gen {
   state: Type;
@@ -475,69 +76,37 @@ Record semantics : Type := Semantics_gen {
   valtype := value_type val_level;
   is_callstate : valtype -> valtype -> state -> Prop;
   step : genvtype -> state -> state -> Prop;
-  (* initial_state: vtype -> vtype -> state -> Prop;*)
   final_state: state -> valtype -> Prop;
   globalenv: genvtype;
-(*  symbolenv: Senv.t *)
 }.
 
 Notation " 'Step' L " := (step L (globalenv L)) (at level 1).
-Notation " 'Star' L " := (star _ _ (step L) (globalenv L)) (at level 1).
-Notation " 'Plus' L " := (plus _ _ (step L) (globalenv L)) (at level 1).
+Notation " 'Star' L " := (star (step L) (globalenv L)) (at level 1).
+Notation " 'Plus' L " := (plus (step L) (globalenv L)) (at level 1).
+
+Definition lift (L : semantics) : FullSemantics.semantics :=
+    {| FullSemantics.state := state L;
+       FullSemantics.genvtype := genvtype L;
+       FullSemantics.val_level := val_level L;
+       FullSemantics.step := fun g s t s' => step L g s s' /\ t = E0;
+       FullSemantics.is_callstate := is_callstate L;
+       FullSemantics.final_state := final_state L;
+       FullSemantics.globalenv := globalenv L;
+       FullSemantics.symbolenv := Genv.to_senv (Genv.empty_genv unit unit nil)
+     |}.
+
+Definition forward_simulation L1 L2 :=
+    forall M, FullSemantics.forward_simulation (lift L1) (lift L2) M.
 
 
 
-Record forward_simulation (L1 L2: semantics) : Type :=
-  Forward_simulation {
-    fsim_index: Type;
-    fsim_order: fsim_index -> fsim_index -> Prop;
-    fsim_order_wf: well_founded fsim_order;
-    fsim_match_states :> fsim_index -> state L1 -> state L2 -> Prop;
-    fsim_match_val : valtype L1 -> valtype L2 -> Prop;
-    fsim_match_callstate :
-      forall fv1 av1 fv2 av2 s2,
-        is_callstate L2 fv2 av2 s2 ->
-        fsim_match_val fv1 fv2 ->
-        fsim_match_val av1 av2 ->
-        exists s1 i,
-          fsim_match_states i s1 s2 /\
-          is_callstate L1 fv1 av1 s1;
-    fsim_match_final_states:
-      forall i s1 s2 v1,
-        fsim_match_states i s1 s2 ->
-        final_state L1 s1 v1 ->
-        exists v2,
-          final_state L2 s2 v2 /\ fsim_match_val v1 v2;
-    fsim_simulation:
-      forall s1 s1', Step L1 s1 s1' ->
-      forall i s2, fsim_match_states i s1 s2 ->
-      exists i', exists s2',
-         (Plus L2 s2 s2' \/ (Star L2 s2 s2' /\ fsim_order i' i))
-      /\ fsim_match_states i' s1' s2';
-(*    fsim_public_preserved:
-      forall id, Senv.public_symbol (symbolenv L2) id = Senv.public_symbol (symbolenv L1) id *)
-    fsim_val_level_le : value_level_le (val_level L1) (val_level L2);
-    fsim_match_val_canon : forall v1 v2,
-        fsim_match_val v1 v2 <->
-        value_match (val_level L1) (val_level L2) v1 v2
-    }.
-
-(** An alternate form of the simulation diagram *)
-
-Lemma fsim_simulation':
-  forall L1 L2 (S: forward_simulation L1 L2),
-  forall i s1 s1', Step L1 s1 s1' ->
-  forall s2, S i s1 s2 ->
-  (exists i', exists s2', Plus L2 s2 s2' /\ S i' s1' s2')
-  \/ (exists i', fsim_order _ _ S i' i /\ S i' s1' s2).
-Proof.
-  intros. exploit fsim_simulation; eauto.
-  intros [i' [s2' [A B]]]. intuition.
-  left; exists i'; exists s2'; auto.
-  inv H2.
-  right; exists i'; auto.
-  left; exists i'; exists s2'; split; auto. econstructor; eauto.
+Lemma lift_notrace_step : forall L s t s',
+    FullSemantics.step (lift L) (globalenv L) s t s' -> t = E0.
+simpl. intros. break_and. eauto.
 Qed.
+
+
+
 
 Section FORWARD_SIMU_DIAGRAMS.
 
@@ -575,11 +144,17 @@ Hypothesis match_val_canon :
     match_values v1 v2 <->
     value_match (val_level L1) (val_level L2) v1 v2.
 
-(** Simulation when one transition in the first program
-    corresponds to zero, one or several transitions in the second program.
-    However, there is no stuttering: infinitely many transitions
-    in the source program must correspond to infinitely many
-    transitions in the second program. *)
+
+Lemma trace_value_level_le : value_level_le_indexed (val_level L1) (val_level L2).
+eapply value_level_le_add_index; eauto.
+Qed.
+
+Lemma trace_match_val_canon : forall M v1 v2,
+    match_values v1 v2 <->
+    value_match_indexed M (val_level L1) (val_level L2) v1 v2.
+intros. rewrite <- value_match_add_index_iff; eauto.
+Qed.
+
 
 Section SIMULATION_STAR_WF.
 
@@ -597,21 +172,26 @@ Hypothesis simulation:
   (Plus L2 s2 s2' \/ (Star L2 s2 s2' /\ order s1' s1))
   /\ match_states s1' s2'.
 
+
 Lemma forward_simulation_star_wf: forward_simulation L1 L2.
 Proof.
-  apply Forward_simulation with
-  (fsim_order := order)
-    (fsim_match_val := match_values)
-    (fsim_match_states := fun idx s1 s2 => idx = s1 /\ match_states s1 s2);
-  auto.
-  intros.
-  exploit match_callstate; eauto.
-  intros. break_exists; break_and.
-  repeat eexists; eauto.
-  intros. destruct H. eapply match_final_states; eauto.
-  intros. destruct H0. subst i. exploit simulation; eauto. intros [s2' [A B]].
-  exists s1'; exists s2'; intuition.
-Defined.
+  intro M. eapply FullSemantics.forward_simulation_star_wf with
+    (order := order)
+    (match_values := match_values)
+    (match_states := match_states);
+  eauto using trace_value_level_le, trace_match_val_canon.
+
+  simpl.
+  intros. break_and. specialize (simulation ?? ** ** ).
+  destruct simulation as (s2' & ? & ?). exists s2'.
+  split; eauto.
+
+  subst t.
+  break_or; [left | right].
+  - eapply lift_plus; eauto.
+  - break_and. split; eauto.
+    eapply lift_star; eauto.
+Qed.
 
 End SIMULATION_STAR_WF.
 
@@ -631,15 +211,23 @@ Hypothesis simulation:
 
 Lemma forward_simulation_star: forward_simulation L1 L2.
 Proof.
-  apply forward_simulation_star_wf with (ltof _ measure).
-  apply well_founded_ltof.
-  intros. exploit simulation; eauto.
-  intros.
-  destruct H1;
-    try break_exists; repeat break_and.
-      exists x; auto.
-  exists s2; split. right; split. apply star_refl. auto. auto.
-Defined.
+  intro M. eapply FullSemantics.forward_simulation_star with
+    (measure := measure)
+    (match_values := match_values)
+    (match_states := match_states);
+  eauto using trace_value_level_le, trace_match_val_canon.
+
+  simpl.
+  intros. break_and. specialize (simulation ?? ** ** ).
+  break_or; [left | right].
+
+  - break_exists. break_and.
+    eexists. split; eauto.
+    subst t.
+    eapply lift_plus; eauto.
+
+  - firstorder eauto.
+Qed.
 
 End SIMULATION_STAR.
 
@@ -655,9 +243,18 @@ Hypothesis simulation:
 
 Lemma forward_simulation_plus: forward_simulation L1 L2.
 Proof.
-  apply forward_simulation_star with (measure := fun _ => O).
-  intros. exploit simulation; eauto.
-Defined.
+  intro M. eapply FullSemantics.forward_simulation_plus with
+    (match_values := match_values)
+    (match_states := match_states);
+  eauto using trace_value_level_le, trace_match_val_canon.
+
+  simpl.
+  intros. break_and. specialize (simulation ?? ** ** ).
+  destruct simulation as (s2' & ? & ?). exists s2'.
+  split; eauto.
+  subst t. eapply lift_plus; eauto.
+
+Qed.
 
 End SIMULATION_PLUS.
 
@@ -673,10 +270,17 @@ Hypothesis simulation:
 
 Lemma forward_simulation_step: forward_simulation L1 L2.
 Proof.
-  apply forward_simulation_plus.
-  intros. exploit simulation; eauto. intros [s2' [A B]].
-  exists s2'; split; auto. apply plus_one; auto.
-Defined.
+  intro M. eapply FullSemantics.forward_simulation_step with
+    (match_values := match_values)
+    (match_states := match_states);
+  eauto using trace_value_level_le, trace_match_val_canon.
+
+  simpl.
+  intros. break_and. specialize (simulation ?? ** ** ).
+  destruct simulation as (s2' & ? & ?). exists s2'.
+  split; eauto.
+
+Qed.
 
 End SIMULATION_STEP.
 
@@ -698,88 +302,27 @@ Hypothesis simulation:
 
 Lemma forward_simulation_opt: forward_simulation L1 L2.
 Proof.
-  apply forward_simulation_star with measure.
-  intros. exploit simulation; eauto.
-  intros [[s2' [A B]] | [A B]].
-  left; exists s2'; split; auto. apply plus_one; auto.
-  right; auto.
-Defined.
+  intro M. eapply FullSemantics.forward_simulation_opt with
+    (match_values := match_values)
+    (match_states := match_states);
+  eauto using trace_value_level_le, trace_match_val_canon.
+
+  simpl.
+  intros. break_and. specialize (simulation ?? ** ** ).
+  break_or; [left | right].
+  - break_exists. break_and.
+    eexists. split; eauto.
+  - firstorder eauto.
+
+Qed.
 
 End SIMULATION_OPT.
 
 End FORWARD_SIMU_DIAGRAMS.
 
-Section SIMULATION_SEQUENCES.
 
-Variable L1: semantics.
-Variable L2: semantics.
-Variable S: forward_simulation L1 L2.
 
-Lemma simulation_star:
-  forall s1 s1', Star L1 s1 s1' ->
-  forall i s2, S i s1 s2 ->
-  exists i', exists s2', Star L2 s2 s2' /\ S i' s1' s2'.
-Proof.
-  induction 1; intros.
-  exists i; exists s2; split; auto. apply star_refl.
-  exploit fsim_simulation; eauto. intros [i' [s2' [A B]]].
-  exploit IHstar; eauto. intros [i'' [s2'' [C D]]].
-  exists i''; exists s2''; split; auto. eapply star_trans; eauto.
-  intuition. apply plus_star; auto.
-Qed.
 
-Lemma simulation_plus:
-  forall s1 s1', Plus L1 s1 s1' ->
-  forall i s2, S i s1 s2 ->
-  (exists i', exists s2', Plus L2 s2 s2' /\ S i' s1' s2')
-  \/ (exists i', clos_trans _ (fsim_order _ _ S) i' i /\ S i' s1' s2).
-Proof.
-  induction 1 using plus_ind2; intros.
-(* base case *)
-  exploit fsim_simulation'; eauto. intros [A | [i' A]].
-  left; auto.
-  right; exists i'; intuition.
-(* inductive case *)
-  exploit fsim_simulation'; eauto. intros [[i' [s2' [A B]]] | [i' [A B]]].
-  exploit simulation_star. apply plus_star; eauto. eauto.
-  intros [i'' [s2'' [P Q]]].
-  left; exists i''; exists s2''; split; auto. eapply plus_star_trans; eauto.
-  exploit IHplus; eauto. intros [[i'' [s2'' [P Q]]] | [i'' [P Q]]].
-  subst. simpl. left; exists i''; exists s2''; auto.
-  subst. simpl. right; exists i''; intuition.
-  eapply t_trans; eauto. eapply t_step; eauto.
-Qed.
-
-(*
-Lemma simulation_forever_silent:
-  forall i s1 s2,
-  Forever_silent L1 s1 -> S i s1 s2 ->
-  Forever_silent L2 s2.
-Proof.
-  assert (forall i s1 s2,
-          Forever_silent L1 s1 -> S i s1 s2 ->
-          forever_silent_N (step L2) (fsim_order S) (globalenv L2) i s2).
-    cofix COINDHYP; intros.
-    inv H. destruct (fsim_simulation S _ _ _ H1 _ _ H0) as [i' [s2' [A B]]].
-    destruct A as [C | [C D]].
-    eapply forever_silent_N_plus; eauto.
-    eapply forever_silent_N_star; eauto.
-  intros. eapply forever_silent_N_forever; eauto. apply fsim_order_wf.
-Qed.
-
-Lemma simulation_forever_reactive:
-  forall i s1 s2 T,
-  Forever_reactive L1 s1 T -> S i s1 s2 ->
-  Forever_reactive L2 s2 T.
-Proof.
-  cofix COINDHYP; intros.
-  inv H.
-  destruct (simulation_star H1 i _ H0) as [i' [st2' [A B]]].
-  econstructor; eauto.
-Qed.
-*)
-
-End SIMULATION_SEQUENCES.
 
 Section COMPOSE_SIMULATIONS.
 
@@ -789,79 +332,10 @@ Variable L3: semantics.
 Variable S12: forward_simulation L1 L2.
 Variable S23: forward_simulation L2 L3.
 
-Let ff_index : Type := (fsim_index _ _ S23 * fsim_index _ _ S12)%type.
-
-Let ff_order : ff_index -> ff_index -> Prop :=
-  lex_ord (clos_trans _ (fsim_order _ _ S23)) (fsim_order _ _ S12).
-
-Let ff_match_states (i: ff_index) (s1: state L1) (s3: state L3) : Prop :=
-  exists s2, S12 (snd i) s1 s2 /\ S23 (fst i) s2 s3.
-
-Let ff_match_values (v1 : valtype L1) (v3 : valtype L3) : Prop :=
-  exists v2, fsim_match_val L1 L2 S12 v1 v2 /\ fsim_match_val L2 L3 S23 v2 v3.
-
 Lemma compose_forward_simulation: forward_simulation L1 L3.
 Proof.
-  apply Forward_simulation with (fsim_order := ff_order) (fsim_match_states := ff_match_states) (fsim_match_val := ff_match_values).
-(* well founded *)
-  unfold ff_order. apply wf_lex_ord. apply wf_clos_trans. apply fsim_order_wf. apply fsim_order_wf.
-(* initial states *)
-  intros. subst ff_match_values. simpl in *. repeat break_exists. repeat break_and.
-  eapply (fsim_match_callstate L2 L3 S23) in H; eauto.
-  repeat break_exists; break_and.
-  eapply (fsim_match_callstate L1 L2 S12) in H4; eauto.
-  break_exists; break_and.
-  exists x3. exists (x2,x4). split; eauto.
-  econstructor; eauto.
-(* final states *)
-  intros. destruct H as [s3 [A B]].
-  app (fsim_match_final_states L1 L2 S12) final_state.
-  app (fsim_match_final_states L2 L3 S23) (final_state L2).
-  eexists; split; try econstructor; eauto.
-(* simulation *)
-  intros. destruct H0 as [s3 [A B]]. destruct i as [i2 i1]; simpl in *.
-  exploit (fsim_simulation' _ _ S12); eauto. intros [[i1' [s3' [C D]]] | [i1' [C D]]].
-  (* L2 makes one or several steps. *)
-  exploit simulation_plus; eauto. intros [[i2' [s2' [P Q]]] | [i2' [P Q]]].
-  (* L3 makes one or several steps *)
-  exists (i2', i1'); exists s2'; split. auto. exists s3'; auto.
-  (* L3 makes no step *)
-  exists (i2', i1'); exists s2; split.
-  right; split. apply star_refl. red. left. auto.
-  exists s3'; auto.
-  (* L2 makes no step *)
-  exists (i2, i1'); exists s2; split.
-  right; split. apply star_refl. red. right. auto.
-  exists s3; auto.
-
-(* value level ordering *)
-  eauto using value_level_le_trans, fsim_val_level_le.
-(* match values canonicalization *)
-  intros. split; intro HH.
-  - destruct HH as (? & ? & ?).
-    eapply value_match_compose; eapply fsim_match_val_canon; eauto.
-  - unfold ff_match_values.
-    destruct (value_match_decompose _ (val_level L2) _ _ _
-            HH (fsim_val_level_le _ _ S12) (fsim_val_level_le _ _ S23))
-        as (? & ? & ?).
-    eexists; split; eapply fsim_match_val_canon; eauto.
-
-(* symbols *)
-  (*  intros. transitivity (Senv.public_symbol (symbolenv L2) id); apply fsim_public_preserved; auto. *)
-Defined.
+    intro M.
+    eapply FullSemantics.compose_forward_simulation; eauto.
+Qed.
 
 End COMPOSE_SIMULATIONS.
-
-Lemma fsim_match_val_compose :
-  forall sema semb semc fs1 fs2 R1 R2,
-    (forall x y, Semantics.fsim_match_val sema semb fs1 x y <-> R1 x y) ->
-    (forall x y, Semantics.fsim_match_val semb semc fs2 x y <-> R2 x y) ->
-    (forall x y, Semantics.fsim_match_val sema semc (Semantics.compose_forward_simulation sema semb semc fs1 fs2) x y <-> (exists z, R1 x z /\ R2 z y)).
-Proof.
-  intros. unfold Semantics.compose_forward_simulation.
-  simpl. split; intros; repeat (break_exists; break_and);
-           repeat rewrite H in *; repeat rewrite H0 in *.
-  eauto.
-  exists x0. split.
-  eapply H; eauto. eapply H0; eauto.
-Qed.
