src/StepLib.v
@@ -110,7 +110,7 @@ Require Semantics.
 
 Lemma sstar_semantics : forall genv state step ge s s',
     sstar (step ge) s s' ->
-    Semantics.star genv state step ge s s'.
+    @Semantics.star genv state step ge s s'.
 induction 1.
 - constructor.
 - econstructor; eauto.
@@ -118,7 +118,7 @@ Qed.
 
 Lemma splus_semantics : forall genv state step ge s s',
     splus (step ge) s s' ->
-    Semantics.plus genv state step ge s s'.
+    @Semantics.plus genv state step ge s s'.
 destruct 1.
 - econstructor; eauto. constructor.
 - econstructor; eauto using splus_sstar, sstar_semantics.
@@ -129,7 +129,7 @@ Lemma splus_semantics_sim : forall genv state_a state_b step
     (exists b' : state_b,
         splus (step ge) b b' /\ match_states a' b') ->
     (exists b' : state_b,
-        Semantics.plus genv state_b step ge b b' /\ match_states a' b').
+        @Semantics.plus genv state_b step ge b b' /\ match_states a' b').
 firstorder eauto using splus_semantics.
 Qed.
 
@@ -139,7 +139,7 @@ Lemma sstar_01_semantics_sim : forall genv state_a state_b step measure
         (step ge b b' \/ (b' = b /\ measure a' < measure a)) /\
         match_states a' b') ->
     ((exists b' : state_b,
-            Semantics.plus genv state_b step ge b b' /\ match_states a' b') \/
+            @Semantics.plus genv state_b step ge b b' /\ match_states a' b') \/
         (measure a' < measure a /\ match_states a' b)).
 intros. break_exists. break_and. on (_ \/ _), invc.
 - left. eapply splus_semantics_sim. firstorder eauto using SPlusOne.
@@ -152,7 +152,7 @@ Lemma sstar_semantics_sim : forall genv state_a state_b step measure
         (splus (step ge) b b' \/ (b' = b /\ measure a' < measure a)) /\
         match_states a' b') ->
     ((exists b' : state_b,
-            Semantics.plus genv state_b step ge b b' /\ match_states a' b') \/
+            @Semantics.plus genv state_b step ge b b' /\ match_states a' b') \/
         (measure a' < measure a /\ match_states a' b)).
 intros. break_exists. break_and. on (_ \/ _), invc.
 - left. eapply splus_semantics_sim. firstorder.
